\documentclass{naproche-library}
\libinput{lists-preamble}
\begin{document}
\begin{smodule}{concatenation.ftl}
  \importmodule[libraries]{lists?lists.ftl}

  \symdef{concat}{\mathop{++}}

  \section*{Concatenation}

  \begin{signature}[forthel,id=LISTS_CONCAT_4578620297183232]
    Let $L, L'$ be lists.
    $L \concat L'$ is a list.
  \end{signature}

  \begin{axiom}[forthel,id=LISTS_CONCAT_3703161885818880]
    Let $L$ be a list.
    Then $\nil \concat L = L$.
  \end{axiom}

  \begin{axiom}[forthel,id=LISTS_CONCAT_8050301789536256]
    Let $a$ be an object and $L, L'$ be lists.
    Then $(a \cons L) \concat L' = a \cons (L \concat L')$.
  \end{axiom}

  \begin{proposition}[forthel,id=LISTS_CONCAT_4512036658964875]
    $L \concat \nil = L$ for every list $L$.
  \end{proposition}
  \begin{proof}[forthel,method=induction on $L$]
    Let $L$ be a list.

    Case $L = \nil$. Trivial.
    
    Case $L = a \cons L'$ for some object $a$ and some list $L'$.
      Consider an object $a$ and a list $L'$ such that $L = a \cons L'$.
      Then $L' \prec L$.
      Hence $L' \concat \nil = L'$.
      Thus $L \concat \nil
        = (a \cons L') \concat \nil
        = a \cons (L' \concat \nil)
        = a \cons L'
        = L$.
    End.
  \end{proof}

  \begin{proposition}[forthel,id=LISTS_CONCAT_1021563255448756]
    $L \concat (L' \concat L'') = (L \concat L') \concat L''$ for any lists $L, L', L''$.
  \end{proposition}
  \begin{proof}[forthel,method=induction on $L$]
    Let $L$ be a list.

    Case $L = \nil$. Trivial.

    Case $L = a \cons L'''$ for some object $a$ and some list $L'''$.
      Consider an object $a$ and a list $L'''$ such that $L = a \cons L'''$.
      Then $L''' \prec L$.
      Let $L',L''$ be lists.
      Then $L''' \concat (L' \concat L'') = (L''' \concat L') \concat L''$.
      [prover vampire]
      Thus $L \concat (L' \concat L'') 
        = (a \cons L''') \concat (L' \concat L'')
        = a \cons (L''' \concat (L' \concat L''))
        = a \cons ((L''' \concat L') \concat L'')
        = (a \cons (L''' \concat L')) \concat L''
        = ((a \cons L''') \concat L') \concat L''
        = (L \concat L') \concat L''$.
    End.
  \end{proof}
\end{smodule}
\end{document}
