\documentclass[10pt]{article}
\usepackage[english]{babel}
\usepackage{../../../../lib/tex/naproche}
\input{../../lib/libraries}
\input{../../lib/lists}
\input{../../lib/arithmetics}
\begin{document}
  \begin{imports}
    \begin{forthel}
      %[prove off][check off]
      [readtex \path{libraries/source/lists/length.ftl.tex}]
      [readtex \path{libraries/source/lists/concatenation.ftl.tex}]
      %[prove on][check on]
    \end{forthel}
  \end{imports}


  \section*{Length of Concatenation}

  \begin{forthel}
    \begin{proposition}\printlabel{LISTS_LENGTHCONCAT_4512036658964875}
      $\length(L \concat L') = \length(L) + \length(L')$ for all lists $L, L'$.
    \end{proposition}
    \begin{proof}[by induction on $L$]
      Let $L$ be a list.

      Case $L = \nil$. Trivial.

      Case $L = a \cons L''$ for some object $a$ and some list $L''$.
        Take an object $a$ and a list $L''$ such that $L = a \cons L''$.
        Then $L'' \prec L$.
        Hence $\length(L'' \concat L') = \length(L'') + \length(L')$ for every list $L'$.
        Thus $\length(L \concat L')
          = \length((a \cons L'') \concat L')
          = \length(a \cons (L'' \concat L'))
          = \length(L'' \concat L') + 1
          = (\length(L'') + \length(L')) + 1
          = (\length(L'') + 1) + \length(L')
          = \length(a \cons L'') + \length(L')
          = \length(L) + \length(L')$
        for every list $L'$.
      End.
    \end{proof}
  \end{forthel}
\end{document}
