\documentclass{naproche-library}
\libinput{lists-preamble}
\begin{document}
\begin{smodule}{reversion.ftl}
  \importmodule[libraries]{lists?concatenation.ftl}

  \symdef{rev}{\textrm{rev}}

  \section*{Reversion}

  \begin{signature}[forthel,id=LISTS_REV_4578620297183232,printid]
    Let $L$ be a list.
    $\rev(L)$ is a list.
  \end{signature}

  \begin{axiom}[forthel,id=LISTS_REV_3703161885818880,printid]
    Let $L$ be a list.
    Then $\rev(\nil) = \nil$.
  \end{axiom}

  \begin{axiom}[forthel,id=LISTS_REV_8050301789536256,printid]
    Let $a$ be an object and $L$ be a list.
    Then $\rev(a \cons L) = \rev(L) \concat [a]$.
  \end{axiom}

  \begin{proposition}[forthel,id=LISTS_REV_4512036658964875,printid]
    $\rev(L \concat L') = \rev(L') \concat \rev(L)$ for any lists $L, L'$.
  \end{proposition}
  \begin{proof}[forthel,method=induction on $L$]
    Let $L,L'$ be lists.

    Case $L = \nil$. Trivial.

    Case $L = a \cons L''$ for some object $a$ and some list $L''$.
      Take an object $a$ and a list $L''$ such that $L = a \cons L''$.
      Then $L'' \prec L$.
      Hence $\rev(L'' \concat L') = \rev(L') \concat \rev(L'')$.
      Thus $\rev(L \concat L')
        = \rev((a \cons L'') \concat L')
        = \rev(a \cons (L'' \concat L'))
        = \rev(L'' \concat L') \concat [a]
        = (\rev(L') \concat \rev(L'')) \concat [a]
        = \rev(L') \concat (\rev(L'') \concat [a])
        = \rev(L') \concat \rev(a \cons L'')
        = \rev(L') \concat \rev(L)$.
      Indeed $(\rev(L') \concat \rev(L'')) \concat [a] = \rev(L') \concat (\rev(L'') \concat [a])$ (by \printref{LISTS_CONCAT_1021563255448756}).
    End.
  \end{proof}

  \begin{proposition}[forthel,id=LISTS_REV_1021563255448756,printid]
    $\rev(\rev(L)) = L$ for every list $L$.
  \end{proposition}
  \begin{proof}[forthel,method=induction on $L$]
    Let $L$ be a list.

    Case $L = \nil$. Trivial.
  
    Case $L = a \cons L'$ for some object $a$ and some list $L'$.
      Take an object $a$ and a list $L'$ such that $L = a \cons L'$.
      Then $L' \prec L$.
      Hence $\rev(\rev(L')) = L'$.
      Thus $\rev(\rev(L))
        = \rev(\rev(a \cons L'))
        = \rev(\rev(L') \concat [a])
        = \rev([a]) \concat \rev(\rev(L'))
        = a \cons \rev(\rev(L'))
        = a \cons L'
        = L$.
    End.
  \end{proof}
\end{smodule}
\end{document}
