\documentclass[../../arithmetic.ftl.tex]{subfiles}

\begin{document}
  \begin{comment}
    \begin{forthel}
      % Uncomment for debugging:

      %[prove off][check off]
      %[readtex arithmetic/sections/01_arithmetic/01_peano-axioms.ftl.tex]
      %[readtex arithmetic/sections/01_arithmetic/02_addition.ftl.tex]
      %[readtex arithmetic/sections/01_arithmetic/03_multiplication.ftl.tex]
      %[readtex arithmetic/sections/01_arithmetic/04_exponentiation.ftl.tex]
      %[readtex arithmetic/sections/01_arithmetic/05_factorial.ftl.tex]
      %[readtex arithmetic/sections/02_ordering/01_ordering.ftl.tex]
      %[readtex arithmetic/sections/02_ordering/02_ordering-and-addition.ftl.tex]
      %[readtex arithmetic/sections/02_ordering/03_ordering-and-multiplication.ftl.tex]
      %[readtex arithmetic/sections/02_ordering/04_ordering-and-exponentiation.ftl.tex]
      %[readtex arithmetic/sections/02_ordering/05_induction.ftl.tex]
      %[readtex arithmetic/sections/02_ordering/06_standard-exercises.ftl.tex]
      %[readtex arithmetic/sections/02_ordering/07_subtraction.ftl.tex]
      %[prove on][check on]
    \end{forthel}
  \end{comment}


  \section{Divisibility}

  \begin{forthel}
    [readtex \path{arithmetic/sections/01_arithmetic/03_multiplication.ftl.tex}]
  \end{forthel}

  \begin{forthel}
    [readtex \path{arithmetic/sections/02_ordering/03_ordering-and-multiplication.ftl.tex}]
  \end{forthel}

  \begin{forthel}
    [readtex \path{arithmetic/sections/02_ordering/04_ordering-and-exponentiation.ftl.tex}]
  \end{forthel}

  \begin{forthel}
    Let $k, l, m, n$ denote natural numbers.
  \end{forthel}


  \subsection{Definitions}

  Just as the standard ordering on the natural numbers determines whether for
  any two natural numbere $n$ and $m$ there exists a natural number $k$ that we
  can add to $n$ to reach $m$, we now do the same with multiplication instead of
  addition. This leads us to the notion of \textit{divisibility}.

  \begin{forthel}
    \begin{definition}
      $n$ divides $m$ iff there exists a natural number $k$ such that $n \cdot k = m$.
    \end{definition}

    \begin{lemma}\label{Arithmetic_03_01_926592}
      $n$ divides $m$ iff there exists a natural number $k$ such that $k \cdot n = m$.
    \end{lemma}

    Let $n \mid m$ stand for $n$ divides $m$.
    Let $m$ is divisible by $n$ stand for $n$ divides $m$.
    Let $n \nmid m$ stand for $n$ does not divide $m$.

    \begin{definition}
      A factor of $n$ is a natural number that divides $n$.
    \end{definition}

    Let a divisor of $n$ stand for a factor of $n$.

    \begin{definition}
      $n$ is even iff $n$ is divisible by $2$.
    \end{definition}

    \begin{definition}
      $n$ is odd iff $n$ is not divisible by $2$.
    \end{definition}
  \end{forthel}


  \subsection{Basic properties}

  As we always did when introducing a new operation or relation, let us now
  prove some basic properties of divisibility.

  \begin{forthel}
    \begin{proposition}\label{Arithmetic_03_01_148842}
      Every natural number divides $0$.
    \end{proposition}
    \begin{proof}
      Let $n$ be a natural number.
      We have $n \cdot 0 = 0$.
      Hence $n \mid 0$.
    \end{proof}

    \begin{proposition}\label{Arithmetic_03_01_295259}
      Every natural number that is divisible by $0$ is equal to $0$.
    \end{proposition}
    \begin{proof}
      Let $n$ be a natural number.
      Assume $0 \mid n$.
      Take a natural number $k$ such that $0 \cdot k = n$.
      Then we have $n = 0$.
    \end{proof}

    \begin{proposition}\label{Arithmetic_03_01_856465}
      $1$ divides every natural number.
    \end{proposition}
    \begin{proof}
      Let $n$ be a natural number.
      We have $1 \cdot n = n$.
      Hence $1 \mid n$.
    \end{proof}

    \begin{proposition}\label{Arithmetic_03_01_258975}
      Every natural number $n$ divides $n$.
    \end{proposition}
    \begin{proof}
      Let $n$ be a natural number.
      We have $n \cdot 1 = n$.
      Hence $n \mid n$.
    \end{proof}

    \begin{proposition}\label{Arithmetic_03_01_211137}
      Every natural number that divides $1$ is equal to $1$.
    \end{proposition}
    \begin{proof}
      Let $n$ be a natural number.
      Assume $n \mid 1$.
      Take a natural number $k$ such that $n \cdot k = 1$.
      Suppose $n \neq 1$.
      Then $n < 1$ or $n > 1$.

      Case $n < 1$.
        Then $n = 0$.
        Hence $0 = 0 \cdot k = n \cdot k = 1$.
        Contradiction.
      End.

      Case $n > 1$.
        We have $k \neq 0$.
        Indeed if $k = 0$ then $1 = n \cdot k = n \cdot 0 = 0$.
        Hence $k \geq 1$.
        Take a positive natural number $l$ such that $n = 1 + l$.
        Then $1 < 1 + l = n = n \cdot 1 \leq n \cdot k$.
        Hence $1 < n$.
        Contradiction.
      End.
    \end{proof}

    \begin{proposition}\label{Arithmetic_03_01_364584}
      We have \[ (\text{$n \mid m$ and $m \mid k$}) \implies n \mid k. \]
    \end{proposition}
    \begin{proof}
      Assume $n \mid m$ and $m \mid k$.
      Take natural numbers $l,l'$ such that $n \cdot l = m$ and $m \cdot l' = k$.
      Then $n \cdot (l \cdot l') = (n \cdot l) \cdot l' = m \cdot l' = k$.
      Hence $n \mid k$.
    \end{proof}

    \begin{proposition}\label{Arithmetic_03_01_185910}
      Let $n$ be nonzero.
      Assume $n \mid m$ and $m \mid n$.
      Then $n = m$.
    \end{proposition}
    \begin{proof}
      Take natural numbers $k,k'$ such that $n \cdot k = m$ and $m \cdot k' = n$.
      Then $n = m \cdot k' = (n \cdot k) \cdot k' = n \cdot (k \cdot k')$.
      Hence $k \cdot k' = 1$.
      Thus $k = 1 = k'$.
      Therefore $n = m$.
    \end{proof}

    \begin{proposition}\label{Arithmetic_03_01_710814}
      We have \[ n \mid m \implies k \cdot n \mid k \cdot m. \]
    \end{proposition}
    \begin{proof}
      Assume $n \mid m$.
      Take a natural number $l$ such that $n \cdot l = m$.
      Then $(k \cdot n) \cdot l = k \cdot (n \cdot l) = k \cdot m$.
      Hence $k \cdot n \mid k \cdot m$.
    \end{proof}

    \begin{proposition}\label{Arithmetic_03_01_382863}
      Assume $k \neq 0$.
      Then \[ k \cdot n \mid k \cdot m \implies n \mid m. \]
    \end{proposition}
    \begin{proof}
      Assume $k \cdot n \mid k \cdot m$.
      Take a natural number $l$ such that $(k \cdot n) \cdot l = k \cdot m$.
      Then $k \cdot (n \cdot l) = k \cdot m$.
      Hence $n \cdot l = m$.
      Thus $n \mid m$.
    \end{proof}

    \begin{proposition}\label{Arithmetic_03_01_210721}
      If $k \mid n$ and $k \mid m$ then $k \mid (n' \cdot n) + (m' \cdot m)$ for all natural numbers $n',m'$.
    \end{proposition}
    \begin{proof}
      Assume $k \mid n$ and $k \mid m$.
      Let $n',m'$ be natural numbers.
      Take natural numbers $l,l'$ such that $k \cdot l = n$ and $k \cdot l' = m$.
      Then

      \[   k \cdot ((n' \cdot l) + (m' \cdot l')) \]
      \[ = (k \cdot (n' \cdot l)) + (k \cdot (m' \cdot l')) \]
      \[ = ((k \cdot n') \cdot l) + ((k \cdot m') \cdot l') \]
      \[ = (n' \cdot (k \cdot l)) + (m' \cdot (k \cdot l')) \]
      \[ = (n' \cdot n) + (m' \cdot m). \]
    \end{proof}

    \begin{corollary}\label{Arithmetic_03_01_655411}
      We have \[ (\text{$k \mid n$ and $k \mid m$}) \implies k \mid n + m. \]
    \end{corollary}
    \begin{proof}
      Assume $k \mid n$ and $k \mid m$.
      Take $n' = 1$ and $m' = 1$.
      Then $k \mid (n' \cdot n) + (m' \cdot m)$ (by \ref{Arithmetic_03_01_210721}).
      $(n' \cdot n) + (m' \cdot m) = n + m$.
      Hence $k \mid n + m$.
    \end{proof}

    \begin{proposition}\label{Arithmetic_03_01_695362}
      Assume $k \mid n$ and $k \mid n + m$.
      Then $k \mid m$.
    \end{proposition}
    \begin{proof}
      Case $k = 0$. Obvious.

      Case $k \neq 0$.
        Take a natural number $l$ such that $n = k \cdot l$.
        Take a natural number $l'$ such that $n + m = k \cdot l'$.
        Then $(k \cdot l) + m = k \cdot l'$.
        We have $l' \geq l$.
        Indeed if $l' < l$ then $n + m = k \cdot l' < k \cdot l = n$.
        Hence we can take a natural number $l''$ such that $l' = l + l''$.
        Then $(k \cdot l) + m = k \cdot l' = k \cdot (l + l'') = (k \cdot l) + (k \cdot l'')$ (by \ref{Arithmetic_01_03_539933}).
        Thus $m = (k \cdot l'')$.
        Therefore $k \mid m$.
      End.
    \end{proof}

    \begin{proposition}\label{Arithmetic_03_01_376821}
      Let $n,m$ be nonzero.
      If $m \mid n$ then $m \leq n$.
    \end{proposition}
    \begin{proof}
      Assume $m \mid n$.
      Take a natural number $k$ such that $m \cdot k = n$.
      If $k = 0$ then $n = m \cdot k = m \cdot 0 = 0$.
      Thus $k \geq 1$.
      Assume $m > n$.
      Then $n = m \cdot k \geq m \cdot 1 = m > n$.
      Hence $n > n$.
      Contradiction.
    \end{proof}

    \begin{proposition}\label{Arithmetic_03_01_499003}
      Let $n,m$ be nonzero and $k > 1$.
      Then $k^{n} \mid k^{m}$ iff $n \leq m$.
    \end{proposition}
    \begin{proof}
      Case $k^{n} \mid k^{m}$.
        Assume $n > m$.
        Take a nonzero natural number $l$ such that $n = m + l$.
        Then $k^{n} = k^{m + l} = k^{m} \cdot k^{l}$.
        Hence $k^{m} \mid k^{n}$.
        Thus $k^{m} = k^{n}$.
        Therefore $m = n$ (by \ref{Arithmetic_02_04_837306}).
        Contradiction.
      End.

      Case $n \leq m$.
        Take a natural number $l$ such that $m = n + l$.
        Then $k^{m} = k^{n + l} = k^{n} \cdot k^{l}$.
        Hence $k^{n} \mid k^{m}$.
      End.
    \end{proof}
  \end{forthel}
\end{document}
