\documentclass{stex}
\libusepackage{naproche}
\libusepackage{copyright}
\libinput{preamble}

\newcommand{\varzero}{x_0}
\newcommand{\abs}[2]{\lambda#1.\ #2}
\newcommand{\app}[2]{(#1)(#2)}
\newcommand{\fix}{\texttt{fix}}

\title{Curry's Paradox in \Naproche}
\author{Marcel Schütz}
\date{2025}

\begin{document}
\begin{smodule}{curry-paradox.ftl}
\maketitle

\noindent \emph{Curry's Paradox} is a paradox described by Haskell Curry in 
1942 \cite{Curry1942}.
It allows the derivation of an arbitrary statement from a self-referential 
expression that presupposes its own validity.

\section*{Untyped $\lambda$-Calculus}

\noindent Our formalization of Curry's Paradox in \Naproche is based on an 
untyped $\lambda$-calculus:

\begin{forthel}
  [synonym expression/-s]

  \begin{signature*}
    An expression is a notion.
  \end{signature*}

  Let $E, E'$ denote expressions.

  \begin{signature*}
    A variable is an expression.
  \end{signature*}

  \begin{signature*}
    $\varzero$ is a variable.
  \end{signature*}

  \begin{signature*}[title=Abstraction,id=abstraction]
    Let $x$ be a variable.
    $\abs{x}{E}$ is an expression.
  \end{signature*}

  \begin{signature*}[title=Application,id=application]
    $\app{E}{E'}$ is an expression.
  \end{signature*}

  \begin{signature*}[title=Fixed-point combinator,id=fixed_point_combinator]
    $\fix$ is an expression such that
    \[\app{\fix}{E} = \app{E}{\app{\fix}{E}}\]
    for every expression $E$.
  \end{signature*}
\end{forthel}


\section*{Propositional Logic}

\noindent We extend this $\lambda$-calculus by a fragment of propositional
logic:

\begin{forthel}  
  Let $E, E'$ denote expressions.
  Let $x$ denote a variable.

  \begin{signature*}[title=Implication,id=implication]
    $E \rightarrow E'$ is an expression.
  \end{signature*}

  \begin{signature*}[title=Truth,id=truth]
    $E$ is true is a relation.
  \end{signature*}

  \begin{axiom*}[title=$\beta$-reduction,id=beta_reduction]
    $\app{\abs{x}{x \rightarrow E'}}{E} = E \rightarrow E'$.
  \end{axiom*}

  \begin{axiom*}[title=Reflexivity,id=reflexivity]
    $E \rightarrow E$ is true.
  \end{axiom*}

  \begin{axiom*}[title=Modus Ponens,id=modus_ponens]
    If $E$ is true and $E \rightarrow E'$ is true then $E'$ is true.
  \end{axiom*}

  \begin{axiom*}[title=Strengthening,id=strengthening]
    If $E \rightarrow (E \rightarrow E')$ is true then $E \rightarrow E'$ is true.
  \end{axiom*}
\end{forthel}


\section*{Curry's paradox}

\noindent Using the fixpoint combinator from above we can formulate a 
self-referential expression $X$ of the form ``If $X$ is true then $E$ is
true'' for any arbitrary expression $E$ by defining
$X = \app{\fix}{\abs{\varzero}{\varzero \rightarrow E}}$.
From the existence of such an expression $X$ together with the above axioms 
we can then derive that any expression $E$ is true.

\begin{forthel}
  \begin{theorem*}[title=Curry's Paradox,id=curry_paradox]
    Every expression is true.
  \end{theorem*}
  \begin{proof}
    Let $E$ be an expression.
    Take $N = \abs{\varzero}{\varzero \rightarrow E}$ and $X = \app{\fix}{N}.$

    (1) Then $X = \app{N}{X} = X \rightarrow E$ (by \nameref{beta_reduction}).

    Hence $X \rightarrow (X \rightarrow E)$ is true (by 1, \nameref{reflexivity}).

    (2) Thus $X \rightarrow E$ is true (by \nameref{strengthening}).

    (3) Therefore $X$ is true (by 1, 2).

    Consequently $E$ is true (by \nameref{modus_ponens}, 2, 3).
  \end{proof}
\end{forthel}

\printbibliography
\printlicense[CcByNcSa]{Marcel Schütz (2024--2025)}
\end{smodule}
\end{document}
