\documentclass{naproche-library}
\libinput{foundations-preamble}
\begin{document}
\begin{smodule}{image-and-preimage.ftl}
  \importmodule[libraries]{foundations?maps.ftl}

  \section*{Computation Laws for Images and Preimages}

  \begin{proposition}[forthel,id=FOUNDATIONS_07_5919649206108160,printid]
    Let $A, B$ be classes and $f : A \to B$ and $X \subseteq A$.
    Then $f_{*}(X) = \{ f(x) \mid x \in X \}$.
  \end{proposition}

  \begin{corollary}[forthel,id=FOUNDATIONS_07_5543924730953728,printid]
    Let $A, B$ be classes and $f : A \to B$.
    Then $f_{*}(A) = \range(f)$.
  \end{corollary}

  \begin{corollary}[forthel,id=FOUNDATIONS_07_1818812171157504,printid]
    Let $A, B$ be classes and $f : A \to B$ and $X \subseteq A$.
    Then $f_{*}(X) = \range(f \restriction X)$.
  \end{corollary}

  \begin{proposition}[forthel,id=FOUNDATIONS_07_911395830890496,printid]
    Let $A$ be a class and $X \subseteq A$.
    Then $(\id_{A})_{*}(X) = X$.
  \end{proposition}

  \begin{proposition}[forthel,id=FOUNDATIONS_07_3349817830932480,printid]
    Let $B$ be a class and $Y \subseteq B$.
    Then $(\id_{B})^{*}(Y) = Y$.
  \end{proposition}

  \begin{proposition}[forthel,id=FOUNDATIONS_07_6362984433582080,printid]
    Let $A, B$ be classes and $f : A \to B$ and $Y \subseteq B$ and $a \in A$.
    Then $f(a) \in Y$ iff $a \in f^{*}(Y)$.
  \end{proposition}
  \begin{proof}[forthel]
    We have $f^{*}(Y) = \{ x \in A \mid f(x) \in Y \}$.
    Hence $a \in f^{*}(Y)$ iff $a \in A$ and $f(a) \in Y$.
    Then we have the thesis.
  \end{proof}

  \begin{proposition}[forthel,id=FOUNDATIONS_07_6730546254184448,printid]
    Let $A, B$ be classes and $f : A \to B$.
    Then $f_{*}(A) \subseteq B$.
  \end{proposition}
  \begin{proof}[forthel]
    $f_{*}(A)
      = f_{*}(\dom(f))
      = \range(f)
      \subseteq B$.
  \end{proof}

  \begin{proposition}[forthel,id=FOUNDATIONS_07_6541963008409600,printid]
    Let $A, B$ be classes and $f : A \to B$.
    Then $f^{*}(B) = A$.
  \end{proposition}
  \begin{proof}[forthel]
    We have $f^{*}(B) = \{ a \in A \mid f(a) \in B \}$.
    $f(a) \in B$ for all $a \in A$.
    Hence the thesis.
  \end{proof}

  \begin{proposition}[forthel,id=FOUNDATIONS_07_1913313581596672,printid]
    Let $A, B$ be classes and $f : A \to B$.
    Then $f_{*}(f^{*}(B)) = f_{*}(A)$.
  \end{proposition}
  \begin{proof}[forthel]
    Let us show that $f_{*}(f^{*}(B)) \subseteq f_{*}(A)$.
      Let $b \in f_{*}(f^{*}(B))$.
      Take $a \in f^{*}(B) \cap A$ such that $b = f(a)$.
      Then $a \in A$.
      Hence $b \in f_{*}(A)$.
    End.

    Let us show that $f_{*}(A) \subseteq f_{*}(f^{*}(B))$.
      Let $b \in f_{*}(A)$.
      Take $a \in A$ such that $b = f(a)$.
      We have $b \in B$.
      Hence $a \in f^{*}(B)$.
      Thus $f(a) \in f_{*}(f^{*}(B))$.
      Indeed $f^{*}(B) \subseteq A$.
      Therefore $b \in f_{*}(f^{*}(B))$.
    End.
  \end{proof}

  \begin{proposition}[forthel,id=FOUNDATIONS_07_3819758101200896,printid]
    Let $A, B$ be classes and $f : A \to B$.
    Then $f^{*}(f_{*}(A)) = A$.
  \end{proposition}
  \begin{proof}[forthel]
    $f^{*}(f_{*}(A)) = \{ a \in A \mid f(a) \in f_{*}(A) \}$.
    For all $a \in A$ we have $f(a) \in f_{*}(A)$.
    Hence every element of $f^{*}(f_{*}(A))$ is contained in $A$ and every element of $A$ is contained in $f^{*}(f_{*}(A))$.
    Thus $f^{*}(f_{*}(A)) = A$.
  \end{proof}

  \begin{proposition}[forthel,id=FOUNDATIONS_07_7760514696347648,printid]
    Let $A, B$ be classes and $f : A \to B$ and $Y \subseteq B$.
    Then $f_{*}(f^{*}(Y)) = Y \cap f_{*}(A)$.
  \end{proposition}
  \begin{proof}[forthel]
    Let us show that $f_{*}(f^{*}(Y)) \subseteq Y \cap f_{*}(A)$.
      Let $b \in f_{*}(f^{*}(Y))$.
      Take $a \in f^{*}(Y)$ such that $b = f(a)$.
      Then $f(a) \in Y \cap f_{*}(A)$.
      Hence we have $b \in Y \cap f_{*}(A)$.
    End.

    Let us show that $Y \cap f_{*}(A) \subseteq f_{*}(f^{*}(Y))$.
      Let $b \in Y \cap f_{*}(A)$.
      Take $a \in A$ such that $b = f(a)$.
      Then $a \in f^{*}(Y)$.
      Hence $f(a) \in f_{*}(f^{*}(Y))$.
    End.
  \end{proof}

  \begin{corollary}[forthel,id=FOUNDATIONS_07_5585105345052672,printid]
    Let $A, B$ be classes and $f : A \to B$ and $Y \subseteq B$.
    Then $f_{*}(f^{*}(Y)) \subseteq Y$.
  \end{corollary}

  \begin{proposition}[forthel,id=FOUNDATIONS_07_4890896170483712,printid]
    Let $A, B$ be classes and $f : A \to B$ and $X \subseteq A$.
    Then $f^{*}(f_{*}(X)) \supseteq X$.
  \end{proposition}
  \begin{proof}[forthel]
    Let $a \in X$.
    Then $f(a) \in f_{*}(X)$.
    Hence $a \in f^{*}(f_{*}(X))$.
    Indeed $f_{*}(X) \subseteq B$.
  \end{proof}

  \begin{proposition}[forthel,id=FOUNDATIONS_07_3318372355801088,printid]
    Let $A, B$ be classes and $f : A \to B$ and $X \subseteq A$.
    Then $f_{*}(X) = \emptyset$ iff $X = \emptyset$.
  \end{proposition}
  \begin{proof}[forthel]
    Case $f_{*}(X)$ is empty.
      Then there is no $a \in X$ such that $f(a) \in f_{*}(X)$.
      For all $a \in X$ we have $f(a) \in f_{*}(X)$.
      Hence $X$ is empty.
    End.

    Case $X$ is empty.
      For all $b \in f_{*}(X)$ we have $b = f(a)$ for some $a \in X$.
      There is no $a \in X$.
      Hence $f_{*}(X)$ is empty.
    End.
  \end{proof}

  \begin{proposition}[forthel,id=FOUNDATIONS_07_8597874786959360,printid]
    Let $A, B$ be classes and $f : A \to B$ and $Y \subseteq B$.
    Then $f^{*}(Y) = \emptyset$ iff $Y \subseteq B \setminus f_{*}(A)$.
  \end{proposition}
  \begin{proof}[forthel]
    Case $f^{*}(Y)$ is empty.
      Let $b \in Y$.
      Then $b \in B$.

      There is no $a \in A$ such that $b = f(a)$. \\
      Proof.
        Assume the contrary.
        Take $a \in A$ such that $b = f(a)$.
        Then $a \in f^{*}(Y)$.
        Contradiction.
      Qed.

      Hence $b \notin f_{*}(A)$.
      Therefore $b \in B \setminus f_{*}(A)$.
    End.

    Case $Y \subseteq B \setminus f_{*}(A)$.
      Then no element of $Y$ is an element of $f_{*}(A)$.
      Assume that $f^{*}(Y)$ is nonempty.
      Take $a \in f^{*}(Y)$.
      Then $f(a) \in Y$ and $f(a) \in f_{*}(A)$.
      Contradiction.
    End.
  \end{proof}

  \begin{proposition}[forthel,id=FOUNDATIONS_07_6295504988143616,printid]
    Let $A, B$ be classes and $f : A \to B$ and $X \subseteq A$ and $Y \subseteq B$.
    Then $f_{*}(X) \cap Y = \emptyset$ iff $X \cap f^{*}(Y) = \emptyset$.
  \end{proposition}
  \begin{proof}[forthel]
    Case $f_{*}(X) \cap Y$ is empty.
      Assume that $X \cap f^{*}(Y)$ is nonempty.
      Take $a \in X \cap f^{*}(Y)$.
      Then $f(a) \in f_{*}(X)$ and $f(a) \in Y$.
      Hence $f(a) \in f_{*}(X) \cap Y$.
      Contradiction.
    End.

    Case $X \cap f^{*}(Y)$ is empty.
      Assume that $f_{*}(X) \cap Y$ is nonempty.
      Take $b \in f_{*}(X) \cap Y$.
      Consider a $a \in X$ such that $b = f(a)$.
      Then $a \in f^{*}(Y)$.
      Indeed $b \in Y$.
      Hence $a \in X \cap f^{*}(Y)$.
      Contradiction.
    End.
  \end{proof}

  \begin{proposition}[forthel,id=FOUNDATIONS_07_5628919411638272,printid]
    Let $A, B, C$ be classes and $f : A \to B$ and $g : B \to C$ and $X \subseteq A$.
    Then $(g \circ f)_{*}(X) = g_{*}(f_{*}(X))$.
  \end{proposition}
  \begin{proof}[forthel]
    $((g \circ f)_{*}(X)) = \{ g(f(a)) \mid a \in X \}$. %!
    $f_{*}(X)$ is a subclass of $B$.
    We have $g_{*}(f_{*}(X)) = \{ g(b) \mid b \in f_{*}(X) \}$ and $f_{*}(X) = \{ f(a) \mid a \in X \}$.
    Thus $g_{*}(f_{*}(X)) = \{ g(f(a)) \mid a \in X \}$.
    Therefore $(g \circ f)_{*}(X) = g_{*}(f_{*}(X))$.
  \end{proof}

  \begin{proposition}[forthel,id=FOUNDATIONS_07_6824917886566400,printid]
    Let $A, B, C$ be classes and $f : A \to B$ and $g : B \to C$ and $Z \subseteq C$.
    Then $(g \circ f)^{*}(Z) = f^{*}(g^{*}(Z))$.
  \end{proposition}
  \begin{proof}[forthel]
    $((g \circ f)^{*}(Z)) = \{ a \in A \mid g(f(a)) \in Z \}$.
    We have $g^{*}(Z) = \{ b \in B \mid g(b) \in Z \}$ and $f^{*}(g^{*}(Z)) = \{ a \in A \mid f(a) \in g^{*}(Z) \}$.
    Hence $f^{*}(g^{*}(Z)) = \{ a \in A \mid g(f(a)) \in Z \}$.
    Thus $(g \circ f)^{*}(Z) = f^{*}(g^{*}(Z))$.
  \end{proof}

  \begin{proposition}[forthel,id=FOUNDATIONS_07_7396318576115712,printid]
    Let $A, B$ be classes and $f : A \to B$ and $X, X' \subseteq A$.
    If $X \subseteq X'$ then $f_{*}(X) \subseteq f_{*}(X')$.
  \end{proposition}
  \begin{proof}[forthel]
    Assume $X \subseteq X'$.
    Let $b \in f_{*}(X)$.
    Take $a \in X$ such that $f(a) = b$.
    Then $a \in X'$.
    Hence $b = f(a) \in f_{*}(X')$.
  \end{proof}

  \begin{proposition}[forthel,id=FOUNDATIONS_07_8376448628817920,printid]
    Let $A, B$ be classes and $f : A \to B$ and $Y, Y' \subseteq B$.
    If $Y \subseteq Y'$ then $f^{*}(Y) \subseteq f^{*}(Y')$.
  \end{proposition}
  \begin{proof}[forthel]
    Assume $Y \subseteq Y'$.
    Let $a \in f^{*}(Y)$.
    Then $f(a) \in Y$.
    Hence $f(a) \in Y'$.
    Thus $a \in f^{*}(Y')$.
  \end{proof}

  \begin{proposition}[forthel,id=FOUNDATIONS_07_4448961469349888,printid]
    Let $A, B$ be classes and $f : A \to B$ and $X, X' \subseteq A$.
    Then $f_{*}(X \cup X') = f_{*}(X) \cup f_{*}(X')$.
  \end{proposition}
  \begin{proof}[forthel]
    Let us show that $f_{*}(X \cup X') \subseteq f_{*}(X) \cup f_{*}(X')$.
      Let $b \in f_{*}(X \cup X')$.
      Take $a \in X \cup X'$ such that $b = f(a)$.
      Then $a \in X$ or $a \in X'$.
      Hence $f(a) \in f_{*}(X)$ or $f(a) \in f_{*}(X')$.
      Thus $b = f(a) \in f_{*}(X) \cup f_{*}(X')$.
    End.

    Let us show that $f_{*}(X) \cup f_{*}(X') \subseteq f_{*}(X \cup X')$.
      Let $b \in f_{*}(X) \cup f_{*}(X')$.

      Case $b \in f_{*}(X)$.
        Take $a \in X$ such that $b = f(a)$.
        Then $a \in X \cup X'$.
        Hence $b \in f_{*}(X \cup X')$.
      End.

      Case $b \in f_{*}(X')$.
        Take $a \in X'$ such that $b = f(a)$.
        Then $a \in X \cup X'$.
        Hence $b \in f_{*}(X \cup X')$.
      End.
    End.
  \end{proof}

  \begin{proposition}[forthel,id=FOUNDATIONS_07_1547089051910144,printid]
    Let $A, B$ be classes and $f : A \to B$ and $Y, Y' \subseteq B$.
    Then $f^{*}(Y \cup Y') = f^{*}(Y) \cup f^{*}(Y')$.
  \end{proposition}
  \begin{proof}[forthel]
    Let us show that $f^{*}(Y \cup Y') \subseteq f^{*}(Y) \cup f^{*}(Y')$.
      Let $a \in f^{*}(Y \cup Y')$.
      Then $f(a) \in Y \cup Y'$.
      Hence $f(a) \in Y$ or $f(a) \in Y'$.
      If $f(a) \in Y$ then $a \in f^{*}(Y)$.
      If $f(a) \in Y'$ then $a \in f^{*}(Y')$.
      Thus $a \in f^{*}(Y) \cup f^{*}(Y')$.
    End.

    Let us show that $f^{*}(Y) \cup f^{*}(Y') \subseteq f^{*}(Y \cup Y')$.
      Let $a \in f^{*}(Y) \cup f^{*}(Y')$.
      Then $a \in f^{*}(Y)$ or $a \in f^{*}(Y')$.
      If $a \in f^{*}(Y)$ then $f(a) \in Y$.
      If $a \in f^{*}(Y')$ then $f(a) \in Y'$.
      Hence $f(a) \in Y \cup Y'$.
      Thus $a \in f^{*}(Y \cup Y')$.
    End.
  \end{proof}

  \begin{proposition}[forthel,id=FOUNDATIONS_07_3966130473402368,printid]
    Let $A, B$ be classes and $f : A \to B$ and $X, X' \subseteq A$.
    Then $f_{*}(X \cap X') \subseteq f_{*}(X) \cap f_{*}(X')$.
  \end{proposition}
  \begin{proof}[forthel]
    Let $b \in f_{*}(X \cap X')$.
    Take $a \in X \cap X'$ such that $b = f(a)$.
    Then $a \in X$ and $a \in X'$.
    Hence $f(a) \in f_{*}(X)$ and $f(a) \in f_{*}(X')$.
    Thus $b \in f_{*}(X) \cap f_{*}(X)$.
  \end{proof}

  \begin{proposition}[forthel,id=FOUNDATIONS_07_4021844428455936,printid]
    Let $A, B$ be classes and $f : A \to B$ and $Y, Y' \subseteq B$.
    Then $f^{*}(Y \cap Y') = f^{*}(Y) \cap f^{*}(Y')$.
  \end{proposition}
  \begin{proof}[forthel]
    Let us show that $f^{*}(Y \cap Y') \subseteq f^{*}(Y) \cap f^{*}(Y')$.
      Let $a \in f^{*}(Y \cap Y')$.
      Then $f(a) \in Y \cap Y'$.
      Hence $f(a) \in Y$ and $f(a) \in Y'$.
      Thus $a \in f^{*}(Y)$ and $a \in f^{*}(Y')$.
      Therefore $a \in f^{*}(Y) \cap f^{*}(Y')$.
    End.

    Let us show that $f^{*}(Y) \cap f^{*}(Y') \subseteq f^{*}(Y \cap Y')$.
      Let $a \in f^{*}(Y) \cap f^{*}(Y')$.
      Then $a \in f^{*}(Y)$ and $a \in f^{*}(Y')$.
      Hence $f(a) \in Y$ and $f(a) \in Y'$.
      Thus $f(a) \in Y \cap Y'$.
      Therefore $a \in f^{*}(Y \cap Y')$.
    End.
  \end{proof}

  \begin{proposition}[forthel,id=FOUNDATIONS_07_8372256617005056,printid]
    Let $A, B$ be classes and $f : A \to B$ and $X, X' \subseteq A$.
    Then $f_{*}(X \setminus X') \supseteq f_{*}(X) \setminus f_{*}(X')$.
  \end{proposition}
  \begin{proof}[forthel]
    Let $b \in f_{*}(X) \setminus f_{*}(X')$.
    Then $b \in f_{*}(X)$ and $b \notin f_{*}(X')$.
    Take $a \in X$ such that $b = f(a)$.
    If $a \in X'$ then $b \in f_{*}(X')$.
    Hence $a \notin X'$.
    Thus $a \in X \setminus X'$.
    Therefore $b = f(a) \in f_{*}(X \setminus X')$.
  \end{proof}

  \begin{proposition}[forthel,id=FOUNDATIONS_07_6552168641331200,printid]
    Let $A, B$ be classes and $f : A \to B$ and $Y, Y' \subseteq B$.
    Then $f^{*}(Y \setminus Y') = f^{*}(Y) \setminus f^{*}(Y')$.
  \end{proposition}
  \begin{proof}[forthel]
    Let us show that $f^{*}(Y \setminus Y') \subseteq f^{*}(Y) \setminus f^{*}(Y')$.
      Let $a \in f^{*}(Y \setminus Y')$.
      Then $f(a) \in Y \setminus Y'$.
      Hence $f(a) \in Y$ and $f(a) \notin Y'$.
      Thus $a \in f^{*}(Y)$ and $a \notin f^{*}(Y')$.
      Therefore $a \in f^{*}(Y) \setminus f^{*}(Y')$.
    End.

    Let us show that $f^{*}(Y) \setminus f^{*}(Y') \subseteq f^{*}(Y \setminus Y')$.
      Let $a \in f^{*}(Y) \setminus f^{*}(Y')$.
      Then $a \in f^{*}(Y)$ and $a \notin f^{*}(Y')$.
      Hence $f(a) \in Y$ and $f(a) \notin Y'$.
      Thus $f(a) \in Y \setminus Y'$.
      Therefore $a \in f^{*}(Y \setminus Y')$.
    End.
  \end{proof}
\end{smodule}
\end{document}
