\documentclass{naproche-library}
\libinput{preamble}
\begin{document}
\IfInputref{}{\setsectionlevel{section}}
\begin{smodule}[title=Multiplication and Ordering]{multiplication-and-ordering.ftl}
\importmodule[libraries/arithmetics]{multiplication.ftl}
\importmodule[libraries/arithmetics]{ordering.ftl}

\begin{proposition}[forthel,id=ARITHMETIC_06_8817333933965312]
  Let $n, m, k$ be natural numbers.
  Assume $k \neq 0$.
  Then $n < m$ iff $n \cdot k < m \cdot k$.
\end{proposition}
\begin{proof}[forthel]
  Case $n \cdot k < m \cdot k$.
    Define $\Phi = \{ n' \in \Nat \mid$ if $n' \cdot k < m \cdot k$ then $n' < m \}$.

    (1) $\Phi$ contains $0$.

    (2) For all $n' \in \Phi$ we have $n' + 1 \in \Phi$. \newline
    Proof.
      Let $n' \in \Phi$.

      Let us show that if $(n' + 1) \cdot k < m \cdot k$ then $n' + 1 < m$.
        Assume $(n' + 1) \cdot k < m \cdot k$.
        Then $(n' \cdot k) + k < m \cdot k$.
        Hence $n' \cdot k < m \cdot k$.
        Thus $n' < m$.
        Then $n' + 1 \leq m$.
        If $n' + 1 = m$ then $(n' + 1) \cdot k = m \cdot k$.
        Hence $n' + 1 < m$.
      End.
    Qed.

    Therefore every natural number is contained in $\Phi$ (by \printref{ARITHMETIC_01_4764664342773760}).
    Consequently $n < m$.
  End.

  Case $n < m$.
    Take a positive natural number $l$ such that $m = n + l$.
    Then $m \cdot k = (n + l) \cdot k = (n \cdot k) + (l \cdot k)$.
    $l \cdot k$ is positive.
    Hence $n \cdot k < m \cdot k$.
  End.
\end{proof}

\begin{corollary}[forthel,id=ARITHMETIC_06_5048640368279552]
  Let $n, m, k$ be natural numbers.
  Assume $k \neq 0$.
  Then $n < m$ iff $k \cdot n < k \cdot m$.
\end{corollary}
\begin{proof}[forthel]
  The thesis (by \printref{ARITHMETIC_06_8817333933965312}, \printref{ARITHMETIC_06_1764759896588288}).
\end{proof}

\begin{proposition}[forthel,id=ARITHMETIC_06_1826268599287808]
  Let $n, m, k$ be natural numbers.
  If $n, m > k$ then $n \cdot m > k$.
\end{proposition}
\begin{proof}[forthel]
  Define $\Phi = \{ n' \in \Nat \mid$ if $n', m > k$ then $n' \cdot m > k \}$.

  (1) $\Phi$ contains $0$.

  (2) For all $n' \in \Phi$ we have $n' + 1 \in \Phi$. \newline
  Proof.
    Let $n' \in \Phi$.

    Let us show that if $n' + 1, m > k$ then $(n' + 1) \cdot m > k$.
      Assume $n' + 1, m > k$.
      Then $(n' + 1) \cdot m = (n' \cdot m) + m$.
      If $n' = 0$ then
      $(n' \cdot m) + m
        = 0 + m
        = m
        > k$.
      If $n' \neq 0$ then
      $(n' \cdot m) + m
        > m
        > k$.
      Indeed if $n' \neq 0$ then $n' \cdot m > 0$.
      Indeed $m > 0$.
      Hence $(n' + 1) \cdot m > k$.
    Qed.
  Qed.

  Thus every natural number is contained in $\Phi$ (by \printref{ARITHMETIC_01_4764664342773760}).
  Therefore if $n, m > k$ then $n \cdot m > k$.
\end{proof}

\begin{corollary}[forthel,id=ARITHMETIC_06_1751605544222720]
  Let $n, m, k$ be natural numbers.
  If $n \leq m$ then $k \cdot n \leq k \cdot m$.
\end{corollary}

\begin{corollary}[forthel,id=ARITHMETIC_06_3965209318260736]
  Let $n, m, k$ be natural numbers.
  Assume $k \neq 0$.
  If $k \cdot n \leq k \cdot m$ then $n \leq m$.
\end{corollary}
\begin{proof}[forthel]
  If $k \cdot n = k \cdot m$ then $n = m$ (by \printref{ARITHMETIC_06_8575191374364672}).
  If $k \cdot n < k \cdot m$ then $n < m$ (by \printref{ARITHMETIC_06_5048640368279552}).
\end{proof}

\begin{corollary}[forthel,id=ARITHMETIC_06_8946886668976128]
  Let $n, m, k$ be natural numbers.
  If $n \leq m$ then $n \cdot k \leq m \cdot k$.
\end{corollary}

\begin{corollary}[forthel,id=ARITHMETIC_06_4374428949413888]
  Let $n, m, k$ be natural numbers.
  Assume $k \neq 0$.
  If $n \cdot k \leq m \cdot k$ then $n \leq m$.
\end{corollary}

\begin{proposition}[forthel,id=ARITHMETIC_06_8813409145454592]
  Let $n, m, k$ be natural numbers.
  Assume $m > 0$ and $k > 1$.
  Then $k \cdot m > m$.
\end{proposition}
\begin{proof}[forthel]
  Take a natural number $l$ such that $k = l + 2$.
  Then
  \[  k \cdot m                       \]
  \[    = (l + 2) \cdot m             \]
  \[    = (l \cdot m) + (2 \cdot m)   \]
  \[    = (l \cdot m) + (m + m)       \]
  \[    = ((l \cdot m) + m) + m       \]
  \[    = ((l + 1) \cdot m) + m       \]
  \[    \geq 1 + m                    \]
  \[    > m.                          \]
  Indeed $((l + 1) \cdot m) + m \geq 1 + m$.
\end{proof}
\end{smodule}
\end{document}
