\documentclass[10pt]{article}
\usepackage[english]{babel}
\usepackage{../../../../lib/tex/naproche}
\input{../../lib/libraries}
\input{../../lib/foundations}
\input{../../lib/arithmetics}
\begin{document}
  \begin{imports}
    \begin{forthel}
      %[prove off][check off]

      [readtex \path{libraries/source/arithmetics/04_ordering.ftl.tex}]

      %[prove on][check on]
    \end{forthel}
  \end{imports}


  \section{Subtraction}

  \begin{forthel}
    \begin{definition}\printlabel{ARITHMETIC_05_8878757276286976}
      Let $n, m$ be natural numbers such that $n \geq m$.
      $n - m$ is the natural number $k$ such that $n = m + k$.
    \end{definition}

    Let the difference of $n$ and $m$ stand for $n - m$.
  \end{forthel}

  \begin{forthel}
    \begin{proposition}\printlabel{ARITHMETIC_05_874271710642176}
      Let $n, m$ be natural numbers such that $n \geq m$.
      Then \[ n - m = 0 \iff n = m. \]
    \end{proposition}
    \begin{proof}
      Case $n - m = 0$.
        Then $n
          = (n - m) + m
          = 0 + m
          = m$.
      End.

      Case $n = m$.
        We have $(n - m) + m
          = n
          = m
          = 0 + m$.
        Hence $n - m = 0$.
      End.
    \end{proof}
  \end{forthel}

  \begin{forthel}
    \begin{corollary}\printlabel{ARITHMETIC_05_8457713057005568}
      Let $n$ be a natural number.
      Then \[ n - n = 0. \]
    \end{corollary}
  \end{forthel}

  \begin{forthel}
    \begin{proposition}\printlabel{ARITHMETIC_05_8518521570983936}
      Let $n$ be a natural number.
      Then \[ n - 0 = n. \]
    \end{proposition}
    \begin{proof}
      We have $n
        = (n - 0) + 0
        = n - 0$.
    \end{proof}
  \end{forthel}

  \begin{forthel}
    \begin{proposition}\printlabel{ARITHMETIC_05_4222566117933056}
      Let $n, m$ be natural numbers such that $n \geq m$.
      Then \[ n - m \leq n. \]
    \end{proposition}
    \begin{proof}
      We have $(n - m) + m = n$.
      Hence $n - m \leq n$.
    \end{proof}
  \end{forthel}

  \begin{forthel}
    \begin{proposition}\printlabel{ARITHMETIC_05_1269537257291776}
      Let $n, m$ be natural numbers such that $n \geq m$.
      Then \[ 0 \neq m < n \implies n - m < n. \]
    \end{proposition}
    \begin{proof}
      Assume $0 \neq m < n$.
      Suppose $n - m \geq n$.
      We have $(n - m) + m = n$.
      Then $n + m
        = (n - m) + m
        = n
        = n + 0$.
      Hence $m = 0$.
      Contradiction.
    \end{proof}
  \end{forthel}

  \begin{forthel}
    \begin{proposition}\printlabel{ARITHMETIC_05_4767595811045376}
      Let $n, m, k$ be natural numbers such that $n \geq m$.
      Then \[ (n - m) + k = (n + k) - m. \]
    \end{proposition}
    \begin{proof}
      We have
      \[  ((n - m) + k) + m       \]
      \[    = ((n - m) + m) + k   \]
      \[    = n + k               \]
      \[    = ((n + k) - m) + m.  \]

      Hence $(n - m) + k = (n + k) - m$.
    \end{proof}
  \end{forthel}

  \begin{forthel}
    \begin{corollary}\printlabel{ARITHMETIC_05_7578468875239424}
      Let $n, m, k$ be natural numbers such that $n \geq m$.
      Then \[ k + (n - m) = (k + n) - m. \]
    \end{corollary}
  \end{forthel}

  \begin{forthel}
    \begin{proposition}\printlabel{ARITHMETIC_05_7595909347016704}
      Let $n, m, k$ be natural numbers such that $n \geq  m + k$.
      Then \[ (n - m) - k = n - (m + k). \]
    \end{proposition}
    \begin{proof}
      We have
      \[  ((n - m) - k) + (m + k)       \]
      \[    = (((n - m) - k) + k) + m   \]
      \[    = (n - m) + m               \]
      \[    = n                         \]
      \[    = (n - (m + k)) + (m + k).  \]

      Hence $(n - m) - k = n - (m + k)$.
    \end{proof}
  \end{forthel}
\end{document}
