\documentclass[10pt]{article}
\usepackage[english]{babel}
\usepackage{../../../../lib/tex/naproche}
\input{../../lib/libraries}
\input{../../lib/foundations}
\input{../../lib/arithmetics}
\begin{document}
  \begin{imports}
    \begin{forthel}
      %[prove off][check off]
      [readtex \path{libraries/source/arithmetics/05_subtraction.ftl.tex}]
      %[prove on][check on]
    \end{forthel}
  \end{imports}


  \section{Definition of Multiplication}

  \begin{forthel}
    \begin{signature}\printlabel{ARITHMETIC_06_6626346484629504}
      Let $n, m$ be natural numbers.
      $n \cdot m$ is a natural number.
    \end{signature}

    Let the product of $n$ and $m$ stand for $n \cdot m$.
  \end{forthel}

  \begin{forthel}
    \begin{axiom}\printlabel{ARITHMETIC_06_8941041092657152}
      Let $n$ be a natural number.
      Then $n \cdot 0 = 0$.
    \end{axiom}
  \end{forthel}

  \begin{forthel}
    \begin{axiom}\printlabel{ARITHMETIC_06_2211275408932864}
      Let $n, m$ be natural numbers.
      Then $n \cdot (m + 1) = (n \cdot m) + n$.
    \end{axiom}
  \end{forthel}


  \section{Computation Laws}

  \subsection{Distributivity}

  \begin{forthel}
    \begin{proposition}\printlabel{ARITHMETIC_06_9001524774567936}
      Let $n, m, k$ be natural numbers.
      Then \[ n \cdot (m + k) = (n \cdot m) + (n \cdot k). \]
    \end{proposition}
    \begin{proof}
      Define $\Phi = \{ k' \in \Nat \mid n \cdot (m + k') =
      (n \cdot m) + (n \cdot k') \}$.

      (1) $0$ is an element of $\Phi$.
      Indeed $n \cdot (m + 0)
        = n \cdot m
        = (n \cdot m) + 0
        = (n \cdot m) + (n \cdot 0)$.

      (2) For all $k' \in \Phi$ we have $k' + 1 \in \Phi$. \\
      Proof.
        Let $k'\in \Phi$.
        Then
        \[  n \cdot (m + (k' + 1))                  \]
        \[    = n \cdot ((m + k') + 1)              \]
        \[    = (n \cdot (m + k')) + n              \]
        \[    = ((n \cdot m) + (n \cdot k')) + n    \]
        \[    = (n \cdot m) + ((n \cdot k') + n)    \]
        \[    = (n \cdot m) + (n \cdot (k' + 1)).   \]
        Hence $n \cdot (m + (k' + 1)) = (n \cdot m) + (n \cdot (k' + 1))$.
        Thus $k' + 1 \in \Phi$.
      Qed.

      Thus every natural number is contained in $\Phi$.
      Therefore $n \cdot (m + k) = (n \cdot m) + (n \cdot k)$.
    \end{proof}
  \end{forthel}

  \begin{forthel}
    \begin{proposition}\printlabel{ARITHMETIC_06_5742967566368768}
      Let $n, m, k$ be natural numbers.
      Then \[ (n + m) \cdot k = (n \cdot k) + (m \cdot k). \]
    \end{proposition}
    \begin{proof}
      Define $\Phi = \{ k' \in \Nat \mid (n + m) \cdot k' =
      (n \cdot k') + (m \cdot k') \}$.

      (1) $0$ belongs to $\Phi$.
      Indeed $(n + m) \cdot 0
        = 0
        = 0 + 0
        = (n \cdot 0) + (m \cdot 0)$.

      (2) For all $k' \in \Phi$ we have $k' + 1 \in \Phi$. \\
      Proof.
        Let $k' \in \Phi$.
        Then
        \[  (n + m) \cdot (k' + 1)                        \]
        \[    = ((n + m) \cdot k') + (n + m)              \]
        \[    = ((n \cdot k') + (m \cdot k')) + (n + m)   \]
        \[    = (((n \cdot k') + (m \cdot k')) + n) + m   \]
        \[    = ((n \cdot k') + ((m \cdot k') + n)) + m   \]
        \[    = ((n \cdot k') + (n + (m \cdot k'))) + m   \]
        \[    = (((n \cdot k') + n) + (m \cdot k')) + m   \]
        \[    = ((n \cdot k') + n) + ((m \cdot k') + m)   \]
        \[    = (n \cdot (k' + 1)) + (m \cdot (k' + 1)).  \]
        Thus $(n + m) \cdot (k' + 1) = (n \cdot (k' + 1)) + (m \cdot (k' + 1))$.
      Qed.

      Thus every natural number is an element of $\Phi$.
      Therefore $(n + m) \cdot k = (n \cdot k) + (m \cdot k)$.
    \end{proof}
  \end{forthel}


  \subsection{Multiplication with $1$ and $2$}

  \begin{forthel}
    \begin{proposition}\printlabel{ARITHMETIC_06_2910559821365248}
      Let $n$ be a natural number.
      Then \[ n \cdot 1 = n. \]
    \end{proposition}
    \begin{proof}
      $n \cdot 1
        = n \cdot (0 + 1)
        = (n \cdot 0) + n
        = 0 + n
        = n$.
    \end{proof}
  \end{forthel}

  \begin{forthel}
    \begin{corollary}\printlabel{ARITHMETIC_06_5679541582299136}
      Let $n$ be a natural number.
      Then \[ n \cdot 2 = n + n. \]
    \end{corollary}
    \begin{proof}
      $n \cdot 2
        = n \cdot (1 + 1)
        = (n \cdot 1) + n
        = n + n$.
    \end{proof}
  \end{forthel}


  \subsection{Associativity}

  \begin{forthel}
    \begin{proposition}\printlabel{ARITHMETIC_06_347295585402880}
      Let $n, m, k$ be natural numbers.
      Then \[ n \cdot (m \cdot k) = (n \cdot m) \cdot k. \]
    \end{proposition}
    \begin{proof}
      Define $\Phi = \{ k' \in \Nat \mid n \cdot (m \cdot k') =
      (n \cdot m) \cdot k' \}$.

      (1) $0$ is contained in $\Phi$.
      Indeed $n \cdot (m \cdot 0)
        = n \cdot 0
        = 0
        = (n \cdot m) \cdot 0$.

      (2) For all $k' \in \Phi$ we have $k' + 1 \in \Phi$. \\
      Proof.
        Let $k' \in \Phi$.
        Then
        \[  n \cdot (m \cdot (k' + 1))                          \]
        \[    = n \cdot ((m \cdot k') + m)                      \]
        \[    = (n \cdot (m \cdot k')) + (n \cdot m)            \]
        \[    = ((n \cdot m) \cdot k') + (n \cdot m)            \]
        \[    = ((n \cdot m) \cdot k') + ((n \cdot m) \cdot 1)  \]
        \[    = (n \cdot m) \cdot (k' + 1).                     \]
      Qed.

      Hence every natural number is contained in $\Phi$ (by \cref{ARITHMETIC_03_647949900054528}).
      Thus $n \cdot (m \cdot k) = (n \cdot m) \cdot k$.
    \end{proof}
  \end{forthel}


  \subsection{Commutativity}

  \begin{forthel}
    \begin{proposition}\printlabel{ARITHMETIC_06_1764759896588288}
      Let $n, m$ be natural numbers.
      Then \[ n \cdot m = m \cdot n. \]
    \end{proposition}
    \begin{proof}
      Define $\Phi = \{ m' \in \Nat \mid n \cdot m' = m' \cdot n \}$.

      (1) $0$ is contained in $\Phi$. \\
      Proof.
        Define $\Psi = \{ n' \in \Nat \mid n' \cdot 0 = 0 \cdot n' \}$.

        (1a) $0$ is contained in $\Psi$.

        (1b) For all $n' \in \Psi$ we have $n' + 1 \in \Psi$. \\
        Proof.
          Let $n' \in \Psi$.
          Then
          \[ (n' + 1) \cdot 0
            = 0
            = n' \cdot 0
            = 0 \cdot n'
            = (0 \cdot n') + 0
            = 0 \cdot (n' + 1). \]
        Qed.

        Hence every natural number is contained in $\Psi$ (by \cref{ARITHMETIC_03_647949900054528}).
        Thus $n \cdot 0 = 0 \cdot n$.
      Qed.

      (2) $1$ belongs to $\Phi$. \\
      Proof.
        Define $\Theta = \{ n' \in \Nat \mid n' \cdot 1 = 1 \cdot n' \}$.

        (2a) $0$ is contained in $\Theta$.

        (2b) For all $n' \in \Theta$ we have $n' + 1 \in \Theta$. \\
        Proof.
          Let $n' \in \Theta$.
          Then
          \[  (n' + 1) \cdot 1        \]
          \[    = (n' \cdot 1) + 1    \]
          \[    = (1 \cdot n') + 1    \]
          \[    = 1 \cdot (n' + 1).   \]
        Qed.

        Thus every natural number is contained in $\Theta$ (by \cref{ARITHMETIC_03_647949900054528}).
        Therefore $n \cdot 1 = 1 \cdot n$.
      Qed.

      (3) For all $m' \in \Phi$ we have $m' + 1 \in \Phi$. \\
      Proof.
        Let $m' \in \Phi$.
        Then
        \[  n \cdot (m' + 1)                \]
        \[    = (n \cdot m') + (n \cdot 1)  \]
        \[    = (m' \cdot n) + (1 \cdot n)  \]
        \[    = (1 \cdot n) + (m' \cdot n)  \]
        \[    = (1 + m') \cdot n            \]
        \[    = (m' + 1) \cdot n.           \]
        Indeed $((1 \cdot n) + (m' \cdot n)) = (1 + m') \cdot n$. %!
      Qed.

      Hence every natural number is contained in $\Phi$ (by \cref{ARITHMETIC_03_647949900054528}).
      Thus $n \cdot m = m \cdot n$.
    \end{proof}
  \end{forthel}


  \subsection{Non-Existence of Zero-Divisors}

  \begin{forthel}
    \begin{proposition}\printlabel{ARITHMETIC_06_3843962875936768}
      Let $n, m$ be natural numbers such that $n \cdot m = 0$.
      Then $n = 0$ or $m = 0$.
    \end{proposition}
    \begin{proof}
      Suppose $n, m \neq 0$.
      Take natural numbers $n', m'$ such that $n = (n' + 1)$ and $m = (m' + 1)$.
      Then
      \[  0                                     \]
      \[    = n \cdot m                         \]
      \[    = (n' + 1) \cdot (m' + 1)           \]
      \[    = ((n' + 1) \cdot m') + (n' + 1)    \]
      \[    = (((n' + 1) \cdot m') + n') + 1.   \]
      Indeed $(n' + 1) \cdot (m' + 1) = ((n' + 1) \cdot m') + (n' + 1)$.
      Hence $0 = k + 1$ for some natural number $k$.
      Contradiction.
    \end{proof}
  \end{forthel}


  \subsection{Cancellation}

  \begin{forthel}
    \begin{proposition}\printlabel{ARITHMETIC_06_31055184658432}
      Let $n, m, k$ be natural numbers.
      Assume $k \neq 0$.
      Then \[ n \cdot k = m \cdot k \implies n = m. \]
    \end{proposition}
    \begin{proof}
      Define $\Phi = \{ n' \in \Nat \mid$ for all $m' \in \Nat$ if
      $n' \cdot k = m' \cdot k$ and $k \neq 0$ then $n' = m' \}$.

      (1) $0$ is contained in $\Phi$. \\
      Proof.
        Let $m' \in \Nat$.
        Assume $0 \cdot k = m' \cdot k$ and $k \neq 0$.
        Then $m' \cdot k = 0$.
        Hence $m' = 0$ or $k = 0$.
        Thus $m' = 0$.
      Qed.

      (2) For all $n' \in \Phi$ we have $n' + 1 \in \Phi$. \\
      Proof.
        Let $n' \in \Phi$.

        Let us show that for all $m' \in \Nat$ if $(n' + 1) \cdot k =
        m' \cdot k$ and $k \neq 0$ then $n' + 1 = m'$.
          Let $m' \in \Nat$.
          Assume $(n' + 1) \cdot k = m' \cdot k$ and $k \neq 0$.

          Case $m' = 0$.
            Then $(n' + 1) \cdot k = 0$.
            Hence $n' + 1 = 0$.
            Contradiction.
          End.

          Case $m' \neq 0$.
            Take a natural number $l$ such that $m' = l + 1$.
            Then $(n' + 1) \cdot k = (l + 1) \cdot k$.
            Hence $(n' \cdot k) + k
              = (n' \cdot k) + (1 \cdot k)
              = (n' \cdot k) + k
              = (l + 1) \cdot k
              = (l \cdot k) + (1 \cdot k)
              = (l \cdot k) + k$.
            Thus $n' \cdot k = l \cdot k$ (by \cref{ARITHMETIC_03_3137702874578944}).
            Indeed $n' \cdot k$ and $l \cdot k$ are natural numbers.
            Then we have $n' = l$.
            Indeed if $n' \cdot k = l \cdot k$ and $k \neq 0$ then $n' = l$.
            Therefore $n' + 1 = l + 1 = m'$.
          End.
        End.

        Hence $n' + 1 \in \Phi$.
      Qed.

      Thus every natural number is contained in $\Phi$ (by \cref{ARITHMETIC_03_647949900054528}).
      Therefore if $n \cdot k = m \cdot k$ then $n = m$.
    \end{proof}
  \end{forthel}

  \begin{forthel}
    \begin{corollary}\printlabel{ARITHMETIC_06_8575191374364672}
      Let $n, m, k$ be natural numbers.
      Assume $k \neq 0$.
      Then \[ k \cdot n = k \cdot m \implies n = m. \]
    \end{corollary}
    \begin{proof}
      Assume $k \cdot n = k \cdot m$.
      We have $k \cdot n = n \cdot k$ and $k \cdot m = m \cdot k$.
      Hence $n \cdot k = m \cdot k$.
      Thus $n = m$ (by \cref{ARITHMETIC_06_31055184658432}).
    \end{proof}
  \end{forthel}


  \section{Ordering and Multiplication}

  \begin{forthel}
    \begin{proposition}\printlabel{ARITHMETIC_06_8817333933965312}
      Let $n, m, k$ be natural numbers.
      Assume $k \neq 0$.
      Then \[ n < m \iff n \cdot k < m \cdot k. \]
    \end{proposition}
    \begin{proof}
      Case $n \cdot k < m \cdot k$.
        Define $\Phi = \{ n' \in \Nat \mid$ if $n' \cdot k < m \cdot k$ then
        $n' < m \}$.

        (1) $\Phi$ contains $0$.

        (2) For all $n' \in \Phi$ we have $n' + 1 \in \Phi$. \\
        Proof.
          Let $n' \in \Phi$.

          Let us show that if $(n' + 1) \cdot k < m \cdot k$ then $n' + 1 < m$.
            Assume $(n' + 1) \cdot k < m \cdot k$.
            Then $(n' \cdot k) + k < m \cdot k$.
            Hence $n' \cdot k < m \cdot k$.
            Thus $n' < m$.
            Then $n' + 1 \leq m$.
            If $n' + 1 = m$ then $(n' + 1) \cdot k = m \cdot k$.
            Hence $n' + 1 < m$.
          End.
        Qed.

        Therefore every natural number is contained in $\Phi$ (by \cref{ARITHMETIC_03_647949900054528}).
        Consequently $n < m$.
      End.

      Case $n < m$.
        Take a positive natural number $l$ such that $m = n + l$.
        Then $m \cdot k = (n + l) \cdot k = (n \cdot k) + (l \cdot k)$.
        $l \cdot k$ is positive.
        Hence $n \cdot k < m \cdot k$.
      End.
    \end{proof}
  \end{forthel}

  \begin{forthel}
    \begin{corollary}\printlabel{ARITHMETIC_06_5048640368279552}
      Let $n, m, k$ be natural numbers.
      Assume $k \neq 0$.
      Then \[ n < m \iff k \cdot n < k \cdot m \]
      (by \cref{ARITHMETIC_06_8817333933965312}, \cref{ARITHMETIC_06_1764759896588288}).
    \end{corollary}
  \end{forthel}

  \begin{forthel}
    \begin{proposition}\printlabel{ARITHMETIC_06_1826268599287808}
      Let $n, m, k$ be natural numbers.
      Then \[ n, m > k \implies n \cdot m > k. \]
    \end{proposition}
    \begin{proof}
      Define $\Phi = \{ n' \in \Nat \mid$ if $n', m > k$ then $n' \cdot m > k \}$.

      (1) $\Phi$ contains $0$.

      (2) For all $n' \in \Phi$ we have $n' + 1 \in \Phi$. \\
      Proof.
        Let $n' \in \Phi$.

        Let us show that if $n' + 1, m > k$ then $(n' + 1) \cdot m > k$.
          Assume $n' + 1, m > k$.
          Then $(n' + 1) \cdot m = (n' \cdot m) + m$.
          If $n' = 0$ then
          $(n' \cdot m) + m
            = 0 + m
            = m
            > k$.
          If $n' \neq 0$ then
          $(n' \cdot m) + m
            > m
            > k$.
          Indeed if $n' \neq 0$ then $n' \cdot m > 0$.
          Indeed $m > 0$.
          Hence $(n' + 1) \cdot m > k$.
        Qed.
      Qed.

      Thus every natural number is contained in $\Phi$ (by \cref{ARITHMETIC_03_647949900054528}).
      Therefore if $n, m > k$ then $n \cdot m > k$.
    \end{proof}
  \end{forthel}

  \begin{forthel}
    \begin{corollary}\printlabel{ARITHMETIC_06_1751605544222720}
      Let $n, m, k$ be natural numbers.
      Then \[ n \leq m \implies k \cdot n \leq k \cdot m. \]
    \end{corollary}
  \end{forthel}

  \begin{forthel}
    \begin{corollary}\printlabel{ARITHMETIC_06_3965209318260736}
      Let $n, m, k$ be natural numbers.
      Assume $k \neq 0$.
      Then \[ k \cdot n \leq k \cdot m \implies n \leq m. \]
    \end{corollary}
    \begin{proof}
      Assume $k \cdot n \leq k \cdot m$.
      Case $k \cdot n = k \cdot m$. Obvious.
      Case $k \cdot n < k \cdot m$. Obvious.
    \end{proof}
  \end{forthel}

  \begin{forthel}
    \begin{corollary}\printlabel{ARITHMETIC_06_8946886668976128}
      Let $n, m, k$ be natural numbers.
      Then \[ n \leq m \implies n \cdot k \leq m \cdot k. \]
    \end{corollary}
  \end{forthel}

  \begin{forthel}
    \begin{corollary}\printlabel{ARITHMETIC_06_4374428949413888}
      Let $n, m, k$ be natural numbers.
      Assume $k \neq 0$.
      Then \[ n \cdot k \leq m \cdot k \implies n \leq m. \]
    \end{corollary}
  \end{forthel}

  \begin{forthel}
    \begin{proposition}\printlabel{ARITHMETIC_06_8813409145454592}
      Let $n, m, k$ be natural numbers.
      Assume $m > 0$ and $k > 1$.
      Then $k \cdot m > m$.
    \end{proposition}
    \begin{proof}
      Take a natural number $l$ such that $k = l + 2$.
      Then
      \[  k \cdot m                       \]
      \[    = (l + 2) \cdot m             \]
      \[    = (l \cdot m) + (2 \cdot m)   \]
      \[    = (l \cdot m) + (m + m)       \]
      \[    = ((l \cdot m) + m) + m       \]
      \[    = ((l + 1) \cdot m) + m       \]
      \[    \geq 1 + m                    \]
      \[    > m.                          \]
      Indeed $((l + 1) \cdot m) + m \geq 1 + m$.
    \end{proof}
  \end{forthel}


  \section{Multiplication and Subtraction}

  \begin{forthel}
    \begin{proposition}\printlabel{ARITHMETIC_06_5458841930039296}
      Let $n, m, k$ be natural numbers such that $n \geq m$.
      Then \[ (n - m) \cdot k = (n \cdot k) - (m \cdot k). \]
    \end{proposition}
    \begin{proof}
      We have
      \[  ((n - m) \cdot k) + (m \cdot k)                 \]
      \[    = ((n - m) + m) \cdot k                       \]
      \[    = n \cdot k                                   \]
      \[    = ((n \cdot k) - (m \cdot k)) + (m \cdot k).  \]

      Hence $(n - m) \cdot k = (n \cdot k) - (m \cdot k)$.
    \end{proof}
  \end{forthel}

  \begin{forthel}
    \begin{corollary}\printlabel{ARITHMETIC_06_8461123277815808}
      Let $n, m, k$ be natural numbers such that $n \geq m$.
      Then \[ k \cdot (n - m) = (k \cdot n) - (k \cdot m). \]
    \end{corollary}
  \end{forthel}
\end{document}
