\documentclass[10pt]{article}
\usepackage[english]{babel}
\usepackage{../../../../lib/tex/naproche}
\input{../../lib/libraries}
\input{../../lib/foundations}
\input{../../lib/arithmetics}
\begin{document}
  \begin{imports}
    \begin{forthel}
      %[prove off][check off]
      [readtex \path{libraries/source/arithmetics/06_multiplication.ftl.tex}]
      %[prove on][check on]
    \end{forthel}
  \end{imports}


  \section{Definition of Exponentiation}

  \begin{forthel}
    \begin{signature}\printlabel{ARITHMETIC_13_3663815629602816}
      Let $n, m$ be natural numbers.
      $n^{m}$ is a natural number.
    \end{signature}
  \end{forthel}

  \begin{forthel}
    \begin{axiom}\printlabel{ARITHMETIC_13_5368818025103360}
      Let $n$ be a natural number.
      Then $n^{0} = 1$.
    \end{axiom}
  \end{forthel}

  \begin{forthel}
    \begin{axiom}\printlabel{ARITHMETIC_13_4140498660884480}
      Let $n, m$ be natural numbers.
      Then $n^{m + 1} = n^{m} \cdot n$.
    \end{axiom}
  \end{forthel}


  \section{Computation Laws}

  \subsection{Exponentiation with $0$, $1$ and $2$}

  \begin{forthel}
    \begin{proposition}\printlabel{ARITHMETIC_13_4673644676513792}
      Let $n$ be a natural number.
      Assume $n \neq 0$.
      Then \[ 0^{n} = 0. \]
    \end{proposition}
    \begin{proof}
      Take a natural number $m$ such that $n = m + 1$.
      Then $0^{n}
        = 0^{m + 1}
        = 0^{m} \cdot 0
        = 0$.
      Indeed $0^{m + 1} = 0^{m} \cdot 0$ (by \cref{ARITHMETIC_13_4140498660884480}).
    \end{proof}
  \end{forthel}

  \begin{forthel}
    \begin{proposition}\printlabel{ARITHMETIC_13_7376849881530368}
      Let $n$ be a natural number.
      Then \[ 1^{n} = 1. \]
    \end{proposition}
    \begin{proof}
      Define $\Phi = \{ n' \in \Nat \mid 1^{n'} = 1 \}$.

      (1) $\Phi$ contains $0$.

      (2) For all $n' \in \Phi$ we have $n' + 1 \in \Phi$. \\
      Proof.
        Let $n' \in \Phi$.
        Then $1^{n' + 1}
          = 1^{n'} \cdot 1
          = 1 \cdot 1
          = 1$.
      Qed.

      Hence every natural number is contained in $\Phi$ (by \cref{ARITHMETIC_03_647949900054528}).
      Thus $1^{n} = 1$.
    \end{proof}
  \end{forthel}

  \begin{forthel}
    \begin{proposition}\printlabel{ARITHMETIC_13_4975279749464064}
      Let $n$ be a natural number.
      Then \[ n^{1} = n. \]
    \end{proposition}
    \begin{proof}
      We have $n^{1}
        = n^{0 + 1}
        = n^{0} \cdot n
        = 1 \cdot n
        = n$.
    \end{proof}
  \end{forthel}

  \begin{forthel}
    \begin{proposition}\printlabel{ARITHMETIC_13_8513812055457792}
      Let $n$ be a natural number.
      Then \[ n^{2} = n \cdot n. \]
    \end{proposition}
    \begin{proof}
      We have $n^{2}
        = n^{1 + 1}
        = n^{1} \cdot n
        = n \cdot n$.
    \end{proof}
  \end{forthel}


  \subsection{Sums as Exponents}

  \begin{forthel}
    \begin{proposition}\printlabel{ARITHMETIC_13_8152207530655744}
      Let $n, m, k$ be natural numbers.
      Then \[ k^{n + m} = k^{n} \cdot k^{m}. \]
    \end{proposition}
    \begin{proof}
      Define $\Phi = \{ m' \in \Nat \mid k^{n + m'} = k^{n} \cdot k^{m'} \}$.

      (1) $\Phi$ contains $0$. \\
      Indeed $k^{n + 0}
        = k^{n}
        = k^{n} \cdot 1
        = k^{n} \cdot k^{0}$.

      (2) For all $m' \in \Phi$ we have $m' + 1 \in \Phi$. \\
      Proof.
        Let $m' \in \Phi$.
        Then
        \[  k^{n + (m' + 1)}                  \]
        \[    = k^{(n + m') + 1}              \]
        \[    = k^{n + m'} \cdot k            \]
        \[    = (k^{n} \cdot k^{m'}) \cdot k  \]
        \[    = k^{n} \cdot (k^{m'} \cdot k)  \]
        \[    = k^{n} \cdot k^{m' + 1}.       \]
      Qed.

      Hence every natural number is contained in $\Phi$ (by \cref{ARITHMETIC_03_647949900054528}).
      Thus $k^{n + m} = k^{n} \cdot k^{m}$.
    \end{proof}
  \end{forthel}


  \subsection{Products as Exponents}

  \begin{forthel}
    \begin{proposition}\printlabel{ARITHMETIC_13_7827956571308032}
      Let $n, m, k$ be natural numbers.
      Then \[ n^{m \cdot k} = (n^{m})^{k}. \]
    \end{proposition}
    \begin{proof}
      Define $\Phi = \{ k' \in \Nat \mid n^{m \cdot k'} = (n^{m})^{k'} \}$.

      (1) $\Phi$ contains $0$.
      Indeed $(n^{m})^{0}
        = 1
        = n^{0}
        = n^{m \cdot 0}$.

      (2) For all $k' \in \Phi$ we have $k' + 1 \in \Phi$. \\
      Proof.
        Let $k' \in \Phi$.
        Then
        \[  (n^{m})^{k' + 1}                \]
        \[    = (n^{m})^{k'} \cdot n^{m}    \]
        \[    = n^{m \cdot k'} \cdot n^{m}  \]
        \[    = n^{(m \cdot k') + m}        \]
        \[    = n^{m \cdot (k' + 1)}.       \]
      Qed.

      Therefore every natural number is contained in $\Phi$ (by \cref{ARITHMETIC_03_647949900054528}).
      Consequently $n^{m \cdot k} = (n^{m})^{k}$.
    \end{proof}
  \end{forthel}


  \subsection{Products as Base}

  \begin{forthel}
    \begin{proposition}\printlabel{ARITHMETIC_13_2563032276271104}
      Let $n, m, k$ be natural numbers.
      Then \[ (n \cdot m)^{k} = n^{k} \cdot m^{k}. \]
    \end{proposition}
    \begin{proof}
      Define $\Phi = \{ k' \in \Nat \mid (n \cdot m)^{k'} =
      n^{k'} \cdot m^{k'} \}$.

      (1) $\Phi$ contains $0$.
      Indeed $((n \cdot m)^{0})
        = 1
        = 1 \cdot 1
        = n^{0} \cdot m^{0}$. %!

      (2) For all $k' \in \Phi$ we have $k' + 1 \in \Phi$. \\
      Proof.
        Let $k' \in \Phi$.

        Let us show that $(n^{k'} \cdot m^{k'}) \cdot (n \cdot m) =
        (n^{k'} \cdot n) \cdot (m^{k'} \cdot m)$.
          \[  (n^{k'} \cdot m^{k'}) \cdot (n \cdot m)       \]
          \[    = ((n^{k'} \cdot m^{k'}) \cdot n) \cdot m   \]
          \[    = (n^{k'} \cdot (m^{k'} \cdot n)) \cdot m   \]
          \[    = (n^{k'} \cdot (n \cdot m^{k'})) \cdot m   \]
          \[    = ((n^{k'} \cdot n) \cdot m^{k'}) \cdot m   \]
          \[    = (n^{k'} \cdot n) \cdot (m^{k'} \cdot m).  \]
        Qed.

        Hence
        \[  (n \cdot m)^{k' + 1}                          \]
        \[    = (n \cdot m)^{k'} \cdot (n \cdot m)        \]
        \[    = (n^{k'} \cdot m^{k'}) \cdot (n \cdot m)   \]
        \[    = (n^{k'} \cdot n) \cdot (m^{k'} \cdot m)   \]
        \[    = n^{k' + 1} \cdot m^{k' + 1}.              \]
      Qed.

      Therefore every natural number is contained in $\Phi$ (by \cref{ARITHMETIC_03_647949900054528}).
      Consequently $(n \cdot m)^{k} = n^{k} \cdot m^{k}$.
    \end{proof}
  \end{forthel}


  \subsection{Zeroes of Exponentiation}

  \begin{forthel}
    \begin{proposition}\printlabel{ARITHMETIC_13_3860221447372800}
      Let $n, m$ be natural numbers.
      Then \[ n^{m} = 0 \iff (\text{$n = 0$ and $m \neq 0$}). \]
    \end{proposition}
    \begin{proof}
      Case $n^{m} = 0$.
        Define $\Phi = \{ m' \in \Nat \mid$ if $n^{m'} = 0$ then $n = 0$ and
        $m' \neq 0 \}$.

        (1) $\Phi$ contains $0$.
        Indeed if $n^{0} = 0$ then we have a contradiction.

        (2) For all $m' \in \Phi$ we have $m' + 1 \in \Phi$. \\
        Proof.
          Let $m' \in \Phi$.

          Let us show that if $n^{m' + 1} = 0$ then $n = 0$ and $m' + 1 \neq 0$.
            Assume $n^{m' + 1} = 0$.
            Then $0 = n^{m' + 1} = n^{m'} \cdot n$.
            Hence $n^{m'} = 0$ or $n = 0$.
            We have $m' + 1 \neq 0$ and if $n^{m'} = 0$ then $n = 0$.
            Hence $n = 0$ and $m' + 1 \neq 0$.
          End.
        Qed.

        Thus every natural number is contained in $\Phi$ (by \cref{ARITHMETIC_03_647949900054528}).
        Consequently $m \in \Phi$.
        Therefore $n = 0$ and $m \neq 0$.
      End.

      Case $n = 0$ and $m \neq 0$.
        Take a natural number $k$ such that $m = k + 1$.
        Then $n^{m}
          = n^{k + 1}
          = n^{k} \cdot n
          = 0^{k} \cdot 0
          = 0$.
      End.
    \end{proof}
  \end{forthel}


  \section{Ordering and Exponentiation}

  \begin{forthel}
    \begin{proposition}\printlabel{ARITHMETIC_13_3373702288769024}
      Let $n, m, k$ be natural numbers.
      Assume $k \neq 0$.
      Then \[ n < m \iff n^{k} < m^{k}. \]
    \end{proposition}
    \begin{proof}
      Case $n < m$.
        Define $\Phi = \{ k' \in \Nat \mid$ if $k' > 1$ then
        $n^{k'} < m^{k'} \}$.

        (1) $\Phi$ contains $0$.

        (2) $\Phi$ contains $1$.

        (3) $\Phi$ contains $2$. \\
        Proof.
          Case $n = 0$ or $m = 0$. Obvious.

          Case $n, m \neq 0$.
            Then $n \cdot n
              < n \cdot m
              < m \cdot m$.
            Hence $n^{2}
              = n \cdot n
              < n \cdot m
              < m \cdot m
              = m^{2}$.
          End.
        Qed.

        (4) For all $k' \in \Phi$ we have $k' + 1 \in \Phi$. \\
        Proof.
          Let $k' \in \Phi$.

          Let us show that if $k' + 1 > 1$ then
          $n^{k' + 1} < m^{k' + 1}$.
            Assume $k' + 1 > 1$.
            Then $n^{k'} < m^{k'}$.
            Indeed $k' \neq 0$ and $if k' = 1$ then $n^{k'} < m^{k'}$.

            Case $k' \leq 1$.
              Then $k' = 0$ or $k' = 1$.
              Hence $k' + 1 = 1$ or $k' + 1 = 2$.
              Thus $k' + 1 \in \Phi$.
              Therefore $n^{k' + 1} < m^{k' + 1}$.
            End.

            Case $k' > 1$.
              Case $n = 0$.
                Then $m \neq 0$.
                Hence $n^{k' + 1}
                  = 0
                  < m^{k'} \cdot m
                  = m^{k' + 1}$.
                Thus $n^{k' + 1} < m^{k' + 1}$.
              End.

              Case $n \neq 0$.
                Then $n^{k'} \cdot n
                  < m^{k'} \cdot n
                  < m^{k'} \cdot m$.
                Indeed $n^{k'} < m^{k'} \neq 0$.
                Take $A = n^{k' + 1}$ and $B = m^{k' + 1}$. %!
                Then $A
                  = n^{k' + 1}
                  = n^{k'} \cdot n
                  < m^{k'} \cdot n
                  < m^{k'} \cdot m
                  = m^{k' + 1}
                  = B$.
                Thus $n^{k' + 1} = A < B = m^{k' + 1}$.
              End.
            End.

            Hence $n^{k' + 1} < m^{k' + 1}$.
            Indeed $k' \leq 1$ or $k' > 1$.
          End.

          Thus $k' + 1 \in \Phi$.
        Qed.

        Therefore every natural number is contained in $\Phi$ (by \cref{ARITHMETIC_03_647949900054528}).
        Consequently $n^{k} < m^{k}$.
      End.

      Case $n^{k} < m^{k}$.
        Define $\Psi = \{ k' \in \Nat \mid$ if $n \geq m$ then
        $n^{k'} \geq m^{k'} \}$.

        (1) $\Psi$ contains $0$.

        (2) For all $k' \in \Psi$ we have $k' + 1 \in \Psi$. \\
        Proof.
          Let $k' \in \Psi$.

          Let us show that if $n \geq m$ then $n^{k' + 1} \geq m^{k' + 1}$.
            Assume $n \geq m$.
            Then $n^{k'} \geq m^{k'}$.
            Hence $n^{k'} \cdot n \geq m^{k'} \cdot n \geq m^{k'} \cdot m$.
            Take $A = n^{k' + 1}$ and $B = m^{k' + 1}$. %!
            Thus $A
              = n^{k' + 1}
              = n^{k'} \cdot n
              \geq m^{k'} \cdot n
              \geq m^{k'} \cdot m
              = m^{k' + 1}
              = B$.
            Therefore $n^{k' + 1} = A \geq B = m^{k' + 1}$.
          End.

          Hence $k' + 1 \in \Psi$.
        Qed.

        Thus every natural number is contained in $\Psi$ (by \cref{ARITHMETIC_03_647949900054528}).
        Therefore if $n \geq m$ then $n^{k} \geq m^{k}$.
        Consequently $n < m$.
      End.
    \end{proof}
  \end{forthel}

  \begin{forthel}
    \begin{corollary}\printlabel{ARITHMETIC_13_2797602550579200}
      Let $n, m, k$ be natural numbers.
      Assume $k \neq 0$.
      Then \[ n^{k} = m^{k} \implies n = m. \]
    \end{corollary}
    \begin{proof}
      Assume $n^{k} = m^{k}$.
      Suppose $n \neq m$.
      Then $n < m$ or $m < n$.
      If $n < m$ then $n^{k} < m^{k}$.
      If $m < n$ then $m^{k} < n^{k}$.
      Thus $n^{k} \neq m^{k}$.
      Contradiction.
    \end{proof}
  \end{forthel}

  \begin{forthel}
    \begin{corollary}\printlabel{ARITHMETIC_13_6875081963732992}
      Let $n, m, k$ be natural numbers.
      Assume $k \neq 0$.
      Then \[ n^{k} \leq m^{k} \iff n \leq m. \]
    \end{corollary}
    \begin{proof}
      If $n^{k} < m^{k}$ then $n < m$.
      If $n^{k} = m^{k}$ then $n = m$.
      [prover vampire]
      Hence $n^{k} \leq m^{k} \implies n \leq m$.
      [prover eprover]

      If $n < m$ then $n^{k} < m^{k}$.
      If $n = m$ then $n^{k} = m^{k}$.
      Hence $n \leq m \implies n^{k} \leq m^{k}$.
    \end{proof}
  \end{forthel}

  \begin{forthel}
    \begin{proposition}\printlabel{ARITHMETIC_13_3349764703780864}
      Let $n, m, k$ be natural numbers.
      Assume $k > 1$.
      Then \[ n < m \iff k^{n} < k^{m}. \]
    \end{proposition}
    \begin{proof}
      Case $n < m$.
        Define $\Phi = \{ m' \in \Nat \mid$ if $n < m'$ then
        $k^{n} < k^{m'} \}$.

        (1) $\Phi$ contains $0$.

        (2) For all $m' \in \Phi$ we have $m' + 1 \in \Phi$. \\
        Proof.
          Let $m' \in \Phi$.

          Let us show that if $n < m' + 1$ then $k^{n} < k^{m' + 1}$.
            Assume $n < m' + 1$.
            Then $n \leq m'$.
            We have $k^{m'} \cdot 1 < k^{m'} \cdot k$.
            Indeed $k^{m'} \neq 0$.

            Case $n = m'$.
              Take $A = k^{n}$ and $B = k^{m' + 1}$. %!
              Then $A
                = k^{n}
                = k^{m'}
                < k^{m'} \cdot k
                = k^{m' + 1}
                = B$.
              Hence $k^{n} = A < B = k^{m' + 1}$.
            End.

            Case $n < m'$.
              Take $A = k^{n}$ and $B = k^{m' + 1}$. %!
              Then $A
                = k^{n}
                < k^{m'}
                < k^{m'} \cdot k
                = k^{m' + 1}
                = B$.
              Hence $k^{n} = A < B = k^{m' + 1}$.
            End.
          Qed.
        Qed.

        Hence every natural number is contained in $\Phi$ (by \cref{ARITHMETIC_03_647949900054528}).
        Thus $k^{n} < k^{m}$.
      End.

      Case $k^{n} < k^{m}$.
        Define $\Psi = \{ n' \in \Nat \mid$ if $n' \geq m$ then
        $k^{n'} \geq k^{m} \}$.

        (1) $0$ is contained in $\Psi$.

        (2) For all $n' \in \Psi$ we have $n' + 1 \in \Psi$. \\
        Proof.
          Let $n' \in \Psi$.

          Let us show that if $n' + 1 \geq m$ then $k^{n' + 1} \geq k^{m}$.
            Assume $n' + 1 \geq m$.

            Case $n' + 1 = m$. Obvious.

            Case $n' + 1 > m$.
              Then $n' \geq m$.
              Hence $k^{n'} \geq k^{m}$.
              We have $k^{n'} \cdot 1 \leq k^{n'} \cdot k$.
              Indeed $1 \leq k$ and $k^{n'} \neq 0$.
              Take $A = k^{m}$ and $B = k^{n' + 1}$. %!
              Then $A
                = k^{m}
                \leq k^{n'}
                = k^{n'} \cdot 1
                \leq k^{n'} \cdot k
                = k^{n' + 1}
                = B$.
              Hence $k^{m} = A \leq B = k^{n' + 1}$.
            End.
          Qed.
        Qed.

        Thus every natural number is contained in $\Psi$ (by \cref{ARITHMETIC_03_647949900054528}).
        Therefore if $n \geq m$ then $k^{n} \geq k^{m}$.
        [prover vampire]
        Consequently $n < m$.
      End.
    \end{proof}
  \end{forthel}

  \begin{forthel}
    \begin{corollary}\printlabel{ARITHMETIC_13_6780506905509888}
      Let $n, m, k$ be natural numbers.
      Assume $k > 1$.
      Then \[ k^{n} = k^{m} \implies n = m. \]
    \end{corollary}
    \begin{proof}
      Assume $k^{n} = k^{m}$.
      Suppose $n \neq m$.
      Then $n < m$ or $m < n$.
      If $n < m$ then $k^{n} < k^{m}$.
      If $m < n$ then $k^{m} < k^{n}$.
      Thus $k^{n} \neq k^{m}$.
      Contradiction.
    \end{proof}
  \end{forthel}

  \begin{forthel}
    \begin{corollary}\printlabel{ARITHMETIC_13_2876620253691904}
      Let $n, m, k$ be natural numbers.
      Assume $k > 1$.
      Then \[ n \leq m \iff k^{n} \leq k^{m}. \]
    \end{corollary}
    \begin{proof}
      If $n \leq m$ then $k^{n} \leq k^{m}$.

      Let us show that if $k^{n} \leq k^{m}$ then $n \leq m$.
        Case $k^{n} = k^{m}$. Obvious (by \cref{ARITHMETIC_13_6780506905509888}).
        Case $k^{n} < k^{m}$. Obvious.
      End.
    \end{proof}
  \end{forthel}

  \begin{forthel}
    \begin{proposition}\printlabel{ARITHMETIC_13_6984104377581568}
      Let $n$ be a natural number.
      Then \[ (n + 1)^{2} = (n^{2} + (2 \cdot n)) + 1. \]
    \end{proposition}
    \begin{proof}
      We have
      \[  (n + 1)^{2}                       \]
      \[    = (n + 1) \cdot (n + 1)         \]
      \[    = ((n + 1) \cdot n) + (n + 1)   \]
      \[    = ((n \cdot n) + n) + (n + 1)   \]
      \[    = (n^{2} + n) + (n + 1)         \]
      \[    = ((n^{2} + n) + n) + 1         \]
      \[    = (n^{2} + (n + n)) + 1         \]
      \[    = (n^{2} + (2 \cdot n)) + 1.    \]
    \end{proof}
  \end{forthel}

  \begin{forthel}
    \begin{proposition}\printlabel{ARITHMETIC_13_134060414337024}
      Let $n$ be a natural number.
      Assume $n \geq 3$.
      Then \[ n^{2} > (2 \cdot n) + 1. \]
    \end{proposition}
    \begin{proof}
      Define $\Phi = \{ n' \in \Nat_{\geq 3} \mid n'^{2} > (2 \cdot n') + 1 \}$.

      (1) $\Phi$ contains $3$.
      Indeed $3^{2} > (2 \cdot 3) + 1$.

      (2) For all $n' \in \Phi$ we have $n' + 1 \in \Phi$. \\
      Proof.
        Let $n' \in \Phi$.
        Then $n' \geq 3$.

        (a) $(n'^{2} + (2 \cdot n')) + 1
        > (((2 \cdot n') + 1) + (2 \cdot n')) + 1$.
        Indeed $n'^{2} + (2 \cdot n') > ((2 \cdot n') + 1) + (2 \cdot n')$.

        (b) $(((2 \cdot n') + 1) + (2 \cdot n')) + 1
        > ((2 \cdot n') + (2 \cdot n')) + 1$. \\
        Proof.
          We have $((2 \cdot n') + 1) + (2 \cdot n')
          > (2 \cdot n') + (2 \cdot n')$.
          Indeed $(2 \cdot n') + 1 > 2 \cdot n'$.
        Qed.

        (c) $(2 \cdot (n' + n')) + 1 > (2 \cdot (n' + 1)) + 1$. \\
        Proof.
          We have $n' + n' > n' + 1$ and $2 \neq 0$.
          Thus $2 \cdot (n' + n') > 2 \cdot (n' + 1)$ (by \cref{ARITHMETIC_06_5048640368279552}).
          Indeed $n' + n'$ and $n' + 1$ are natural numbers.
        Qed.

        Take $A = (n' + 1)^{2}$ and $B = (2 \cdot (n' + 1)) + 1$. %!
        Then
        \[  A                                             \]
        \[    = (n' + 1)^{2}                              \]
        \[    = (n'^{2} + (2 \cdot n')) + 1               \]
        \[    > (((2 \cdot n') + 1) + (2 \cdot n')) + 1   \]  % (a)
        \[    > ((2 \cdot n') + (2 \cdot n')) + 1         \]  % (b)
        \[    = (2 \cdot (n' + n')) + 1                   \]
        \[    > (2 \cdot (n' + 1)) + 1                    \]  % (c)
        \[    = B.                                        \]

        Thus $(n' + 1)^{2} = A > B = (2 \cdot (n' + 1)) + 1$.
      Qed.

      [prover vampire]
      Therefore $\Phi$ contains every element of $\Nat_{\geq 3}$ (by \cref{ARITHMETIC_04_4976599269113856}, 1, 2).
      [prover eprover]
      Consequently $n^{2} > (2 \cdot n) + 1$.
    \end{proof}
  \end{forthel}
\end{document}
