\documentclass[10pt]{article}
\usepackage[english]{babel}
\usepackage{../../../../lib/tex/naproche}
\input{../../lib/libraries}
\input{../../lib/foundations}
\input{../../lib/arithmetics}
\begin{document}
  \begin{imports}
    \begin{forthel}
      %[prove off][check off]
      [readtex \path{libraries/source/arithmetics/divisibility.ftl.tex}]
      [readtex \path{libraries/source/arithmetics/subtraction.ftl.tex}]
      %[prove on][check on]
    \end{forthel}
  \end{imports}


  \section*{Even and Odd Numbers}

  \subsection*{Definition}

  \begin{forthel}
    \begin{definition}\printlabel{ARITHMETIC_15_4521358965847512}
      Let $n$ be a natural number.
      $n$ is even iff $n$ is divisible by $2$.
    \end{definition}
  \end{forthel}

  \begin{forthel}
    \begin{definition}\printlabel{ARITHMETIC_15_1023652125874596}
      Let $n$ be a natural number.
      $n$ is odd iff $n$ is not divisible by $2$.
    \end{definition}
  \end{forthel}

  \begin{forthel}
    \begin{proposition}\printlabel{ARITHMETIC_15_0236985458752156}
      Let $n$ be a natural number.
      $n$ is even iff $n = 2 \cdot m$ for some natural number $m$.
    \end{proposition}
    \begin{proof}
      Case $n$ is even.
        Then $2$ divides $n$.
        Hence $n = 2 \cdot m$ for some natural number $m$.
      End.

      Case $n = 2 \cdot m$ for some natural number $m$.
        Then $2$ divides $n$.
        Hence $2$ is even.
      End.
    \end{proof}
  \end{forthel}

  \begin{forthel}
    \begin{proposition}\printlabel{ARITHMETIC_15_1023512547854265}
      Let $n$ be a natural number.
      $n$ is odd iff $n = (2 \cdot m) + 1$ for some natural number $m$.
    \end{proposition}
    \begin{proof}
      Case $n$ is odd.
        (a) Define $\Phi = \{ n' \in \Nat \mid$ if $n'$ is odd then $n' = (2 \cdot m) + 1$ for some natural number $m \}$.

        (1) $\Phi$ contains $0$.
        Indeed $0$ is not odd.

        (2) For all $n' \in \Phi$ we have $n' + 1 \in \Phi$. \\
        Proof.
          Let $n' \in \Phi$.

          Let us show that if $n' + 1$ is odd then $(n' + 1) = (2 \cdot m) + 1$ for some natural number $m$.
            Assume that $n' + 1$ is odd.

            Case $n'$ is even.
              Take a natural number $m$ such that $n' = 2 \cdot m$.
              Then $n' + 1 = (2 \cdot m) + 1$.
            End.

            Case $n'$ is odd.
              Take a natural number $m$ such that $n' = (2 \cdot m) + 1$.
              Then $n' + 1
                = ((2 \cdot m) + 1) + 1
                = (2 \cdot m) + (1 + 1)
                = (2 \cdot m) + 2
                = 2 \cdot (m + 1)$.
              Hence $2$ divides $n'$.
              Thus $n'$ is even.
              Contradiction.
            End.
          End.
        Qed.

        Then $\Phi$ contains every natural number (by \printref{ARITHMETIC_01_4764664342773760}).
        Hence $n$ is odd iff $n = (2 \cdot m) + 1$ for some natural number $m$ (by a).
      End.

      Case $n = (2 \cdot m) + 1$ for some natural number $m$.
        Consider a natural number $m$ such that $n = (2 \cdot m) + 1$.
        Assume that $n$ is even.
        Then we can take a natural number $k$ such that $n = 2 \cdot k$.
        Then we have $2 \cdot k = (2 \cdot m) + 1$.
        Hence $2$ divides $(2 \cdot m) + 1$.
        Thus $2$ divides $1$.
        Indeed $2$ divides $2 \cdot m$.
        Contradiction.
      End.
    \end{proof}
  \end{forthel}

  \begin{forthel}
    \begin{proposition}\printlabel{ARITHMETIC_15_1023652154254789}
      Let $n$ be a natural number.
      $n$ is odd iff $n = (2 \cdot m) - 1$ for some positive natural number $m$.
    \end{proposition}
    \begin{proof}
      Case $n$ is odd.
        Consider a natural number $k$ such that $n = (2 \cdot k) + 1$.
        Take $m = k + 1$.
        Then $n
          = (2 \cdot k) + 1
          = (2 \cdot (k + 0)) + 1
          = (2 \cdot (k + (1 - 1))) + 1
          = (2 \cdot ((k + 1) - 1)) + 1
          = (2 \cdot (m - 1)) + 1
          = ((2 \cdot m) - (2 \cdot 1)) + 1
          = ((2 \cdot m) - 2) + 1
          = (2 \cdot m) - 1$.
      End.

      Case $n = (2 \cdot m) - 1$ for some positive natural number $m$.
        Consider a positive natural number $m$ such that $n = (2 \cdot m) - 1$.
        Take $k = m - 1$.
        Then $n
          = (2 \cdot m) - 1
          = (2 \cdot (m + 0)) - 1
          = (2 \cdot (m + (1 - 1))) - 1
          = (2 \cdot ((m + 1) - 1)) - 1
          = (2 \cdot ((m - 1) + 1)) - 1
          = (2 \cdot (k + 1)) - 1
          = ((2 \cdot k) + (2 \cdot 1)) - 1
          = ((2 \cdot k) + 2) - 1
          = (2 \cdot k) + (2 - 1)
          = (2 \cdot k) + 1$.
        Hence $n$ is odd.
      End.
    \end{proof}
  \end{forthel}


  \subsection*{Addition of Even and Odd Numbers}

  \begin{forthel}
    \begin{proposition}\printlabel{ARITHMETIC_15_7845441256365256}
      Let $n, m$ be natural numbers.
      Assume that $n$ and $m$ are even.
      Then $n + m$ is even.
    \end{proposition}
    \begin{proof}
      Take natural numbers $k, l$ such that $n = 2 \cdot k$ and $m = 2 \cdot l$.
      Then $n + m
        = (2 \cdot k) + (2 \cdot l)
        = 2 \cdot (k + l)$.
      Hence $n + m$ is even.
    \end{proof}
  \end{forthel}

  \begin{forthel}
    \begin{proposition}\printlabel{ARITHMETIC_15_1023655256985478}
      Let $n, m$ be natural numbers.
      Assume that $n$ is even and $m$ is odd.
      Then $n + m$ is odd.
    \end{proposition}
    \begin{proof}
      Take natural numbers $k, l$ such that $n = 2 \cdot k$ and $m = (2 \cdot l) + 1$.
      Then $n + m
        = (2 \cdot k) + ((2 \cdot l) + 1)
        = ((2 \cdot k) + (2 \cdot l)) + 1
        = (2 \cdot (k + l)) + 1$.
      Hence $n + m$ is odd.
    \end{proof}
  \end{forthel}

  \begin{forthel}
    \begin{corollary}\printlabel{ARITHMETIC_15_0125412589658745}
      Let $n, m$ be natural numbers.
      Assume that $n$ is odd and $m$ is even.
      Then $n + m$ is odd.
    \end{corollary}
  \end{forthel}

  \begin{forthel}
    \begin{proposition}\printlabel{ARITHMETIC_15_1023659854785412}
      Let $n, m$ be natural numbers.
      Assume that $n$ and $m$ are odd.
      Then $n + m$ is even.
    \end{proposition}
    \begin{proof}
      Take natural numbers $k, l$ such that $n = (2 \cdot k) + 1$ and $m = (2 \cdot l) + 1$.
      Then $n + m
        = ((2 \cdot k) + 1) + ((2 \cdot l) + 1)
        = (((2 \cdot k) + 1) + (2 \cdot l)) + 1
        = ((2 \cdot k) + (1 + (2 \cdot l))) + 1
        = ((2 \cdot k) + ((2 \cdot l) + 1)) + 1
        = (((2 \cdot k) + (2 \cdot l)) + 1) + 1
        = ((2 \cdot k) + (2 \cdot l)) + (1 + 1)
        = ((2 \cdot k) + (2 \cdot l)) + 2
        = (2 \cdot (k + l)) + 2
        = 2 \cdot ((k + l) + 1)$.
        Hence $n + m$ is even.
    \end{proof}
  \end{forthel}


  \subsection{Subtraction of even and odd numbers}

  \begin{forthel}
    \begin{proposition}\printlabel{ARITHMETIC_15_8748569852145203}
      Let $n, m$ be natural numbers such that $n \geq m$.
      Assume that $n, m$ are even.
      Then $n - m$ is even.
    \end{proposition}
    \begin{proof}
      Take natural numbers $k, l$ such that $n = 2 \cdot k$ and $m = 2 \cdot l$.
      Then $k \geq l$.
      Hence $n - m
        = (2 \cdot k) - (2 \cdot l)
        = 2 \cdot (k - l)$.
      Thus $n - m$ is even.
    \end{proof}
  \end{forthel}

  \begin{forthel}
    \begin{proposition}\printlabel{ARITHMETIC_15_0125412036589958}
      Let $n, m$ be natural numbers such that $n \geq m$.
      Assume that $n$ is even and $m$ is odd.
      Then $n - m$ is odd.
    \end{proposition}
    \begin{proof}
      Take natural numbers $k, l$ such that $n = 2 \cdot k$ and $m = (2 \cdot l) + 1$.
      Then $k \geq l$ and $2 \cdot (k - l) \geq 1$.
      Hence $n - m
        = (2 \cdot k) - ((2 \cdot l) + 1)
        = ((2 \cdot k) - (2 \cdot l)) - 1
        = (2 \cdot (k - l)) - 1$.
      Thus $n - m$ is odd.
    \end{proof}
  \end{forthel}

  \begin{forthel}
    \begin{corollary}\printlabel{ARITHMETIC_15_1021458745896523}
      Let $n, m$ be natural numbers such that $n \geq m$.
      Assume that $n$ is odd and $m$ is even.
      Then $n - m$ is odd.
    \end{corollary}
    \begin{proof}
      Take natural numbers $k, l$ such that $n = (2 \cdot k) + 1$ and $m = 2 \cdot l$.
      Then $k \geq l$.
      Hence $n - m
        = ((2 \cdot k) + 1) - (2 \cdot l)
        = (1 + (2 \cdot k)) - (2 \cdot l)
        = 1 + ((2 \cdot k) - (2 \cdot l))
        = ((2 \cdot k) - (2 \cdot l)) + 1
        = (2 \cdot (k - l)) + 1$.
      Indeed $((2 \cdot k) - (2 \cdot l)) = 2 \cdot (k - l)$. %!
      Thus $n - m$ is odd.
    \end{proof}
  \end{forthel}

  \begin{forthel}
    \begin{proposition}\printlabel{ARITHMETIC_15_0125478854587412}
      Let $n, m$ be natural numbers such that $n \geq m$.
      Assume that $n, m$ are odd.
      Then $n - m$ is even.
    \end{proposition}
    \begin{proof}
      Take natural numbers $k, l$ such that $n = (2 \cdot k) + 1$ and $m = (2 \cdot l) + 1$.
      Then $k \geq l$.
      Indeed $2 \cdot k \geq 2 \cdot l$.
      Hence $1 + (2 \cdot k) \geq 2 \cdot l$.
      Thus $n - m
        = ((2 \cdot k) + 1) - ((2 \cdot l) + 1)
        = ((1 + (2 \cdot k)) - (2 \cdot l)) - 1
        = (1 + ((2 \cdot k) - (2 \cdot l))) - 1
        = (1 + (2 \cdot (k - l))) - 1
        = ((2 \cdot (k - l)) + 1) - 1
        = 2 \cdot (k - l)$.
      Indeed $((2 \cdot k) - (2 \cdot l)) = 2 \cdot (k - l)$. %!
      Therefore $n - m$ is even.
    \end{proof}
  \end{forthel}


  \subsection*{Multiplication of Even and Odd Numbers}

  \begin{forthel}
    \begin{proposition}\printlabel{ARITHMETIC_15_0125698547589652}
      Let $n, m$ be natural numbers.
      Assume that $n$ is even or $n$ is even.
      Then $n \cdot m$ is even.
    \end{proposition}
    \begin{proof}
      Case $n$ is even.
        Take a natural number $k$ such that $n = 2 \cdot k$.
        Then $n \cdot m
          = (2 \cdot k) \cdot m
          = 2 \cdot (k \cdot m)$.
        Hence $n \cdot m$ is even.
      End.

      Case $m$ is even.
        Take a natural number $l$ such that $m = 2 \cdot l$.
        Then $n \cdot m
          = n \cdot (2 \cdot l)
          = (n \cdot 2) \cdot l
          = (2 \cdot n) \cdot l
          = 2 \cdot (n \cdot l)$.
        Hence $n \cdot m$ is even.
      End.
    \end{proof}
  \end{forthel}

  \begin{forthel}
    \begin{proposition}\printlabel{ARITHMETIC_15_0236596587452145}
      Let $n, m$ be natural numbers.
      Assume that $n$ and $m$ are odd.
      Then $n \cdot m$ is odd.
    \end{proposition}
    \begin{proof}
      Take natural numbers $k, l$ such that $n = (2 \cdot k) + 1$ and $m = (2 \cdot l) + 1$.
      Then $n \cdot m
        = ((2 \cdot k) + 1) \cdot m
        = ((2 \cdot k) \cdot m) + (1 \cdot m)
        = ((2 \cdot k) \cdot m) + m
        = (2 \cdot (k \cdot m)) + m$.
      $2 \cdot (k \cdot m)$ is even and $m$ is odd.
      Hence $(2 \cdot (k \cdot m)) + m$ is odd.
      Therefore $n \cdot m$ is odd.
    \end{proof}
  \end{forthel}
\end{document}