\documentclass{naproche-library}
\libinput{arithmetics-preamble}
\begin{document}
\begin{smodule}{exponentiation-and-division.ftl}
  \importmodule[libraries]{arithmetics?division.ftl}
  \importmodule[libraries]{arithmetics?exponentiation.ftl}
  \importmodule[libraries]{arithmetics?subtraction.ftl}

  \section*{Exponentiation and Division}

  \begin{proposition}[forthel,id=ARITHMETIC_14_2345102698451257]
    Let $n, m, k$ be natural numbers such that $k$ is nonzero and $n \geq m$.
    Then \[\frac{k^{n}}{k^{m}} = k^{n - m}.\]
  \end{proposition}
  \begin{proof}[forthel]
    We have $k^{n} = k^{(n - m) + m} = k^{n - m} \cdot k^{m}$.
    Hence
    \[  \frac{k^{n}}{k^{m}}
        = \frac{k^{n - m} \cdot k^{m}}{k^{m}}
        = \frac{k^{n - m} \cdot k^{m}}{1 \cdot k^{m}}
        = \frac{k^{n - m}}{1}
        = k^{n - m}. \]
  \end{proof}
\end{smodule}
\end{document}