\documentclass{naproche-library}
\libinput{arithmetics-preamble}
\begin{document}
\begin{smodule}{multiplication-and-subtraction.ftl}
  \importmodule[libraries]{arithmetics?multiplication.ftl}
  \importmodule[libraries]{arithmetics?subtraction.ftl}

  \section*{Multiplication and Subtraction}

  \begin{proposition}[forthel,id=ARITHMETIC_06_5458841930039296,printid]
    Let $n, m, k$ be natural numbers such that $n \geq m$.
    Then $(n - m) \cdot k = (n \cdot k) - (m \cdot k)$.
  \end{proposition}
  \begin{proof}[forthel]
    We have
    \[  ((n - m) \cdot k) + (m \cdot k)                 \]
    \[    = ((n - m) + m) \cdot k                       \]
    \[    = n \cdot k                                   \]
    \[    = ((n \cdot k) - (m \cdot k)) + (m \cdot k).  \]

    Hence $(n - m) \cdot k = (n \cdot k) - (m \cdot k)$.
  \end{proof}

  \begin{corollary}[forthel,id=ARITHMETIC_06_8461123277815808,printid]
    Let $n, m, k$ be natural numbers such that $n \geq m$.
    Then $k \cdot (n - m) = (k \cdot n) - (k \cdot m)$.
  \end{corollary}
\end{smodule}
\end{document}
